This is a good commit!
Most all of the Omega mapping functions were imported
into Isabelle/HOL through Haskabelle. However, just a few
bits are not yet present. I think I have enough material for now.

Why not all were imported? Verbose with Haskabelle is really poor
- I can't extract any information on why or what is going wrong
with my code.

!!BUT!! I suspect Haskabelle is having a similar though about my code
as Isabelle is when I directly write it into the *.thy file. The following
lines are left as comments in Isabelle since it is showing some sort of error:

(*
| "omega_CAction lst (CActionCommand (CommandBrace g)) = omega_CAction lst (CActionCommand (CPrefix g (ZTrue Nil)))"
| "omega_CAction lst (CActionCommand (CommandBracket g)) = omega_CAction lst (CActionCommand (CPrefix1 g))"
| "omega_CAction lst (CSPCommAction (ChanComm c ((ChanOutExp e) # xs)) a) = omega_CAction lst (CSPCommAction (ChanComm c ((ChanDotExp e) # xs)) a)"
| "omega_CAction lst (CSPCommAction (ChanComm c Nil) a) = (CSPCommAction (ChanComm c Nil) (omega_CAction lst a))"
| "omega_CAction lst (CSPHide a cs) = (CSPHide (omega_CAction lst a) cs)"
| "omega_CAction lst (CSPIntChoice ca cb) = (CSPIntChoice (omega_CAction lst ca) (omega_CAction lst cb))"
| "omega_CAction lst (CSPSeq ca cb) = (CSPSeq (omega_CAction lst ca) (omega_CAction lst cb))"
| "omega_CAction lst (CSPRecursion x c) = (CSPRecursion x (omega_CAction lst c))"
*)

I'll leave them for later evaluation, I think I have enough in my plate
for now.

The file MappingFunStatelessCircus.lhs-orig contains the remainder of
the omega functions.

Next stop: put the refinement laws into Isabelle/HOL - Fingers crossed

test_haskabelle/DefSets.hs
@@ -8,97 +8,87 @@ module DefSets where
 -- import Data.Text hiding (map,concat,all)
 import AST
 
+-- 
+
+filter_state_comp :: [(ZName, ZVar, ZExpr)] -> [ZVar]
+filter_state_comp [] = []
+filter_state_comp [(_, v, _)] = [v]
+filter_state_comp ((_, v, _):xs) = [v]++(filter_state_comp xs)
+
+get_guard_pair :: CGActions -> [(ZPred, CAction)]
+get_guard_pair (CircThenElse (CircGAction g2 a2) (CircGAction g3 a3)) = [(g2,a2),(g3,a3)]
+get_guard_pair (CircThenElse (CircGAction g1 a1) glx) = [(g1,a1)]++(get_guard_pair glx)
 
 
--- TODO: Need to do it
+
+make_get_com :: [(ZName, ZVar, ZExpr)] -> [ZVar] -> CAction -> CAction
+make_get_com lst [(x,[])] c = (CSPCommAction (ChanComm "mget"[ChanDotExp (ZVar ((get_proc_name x lst)++"_"++x,[])),ChanInp ("v"++(get_proc_name x lst)++"_"++x)]) c)
+make_get_com lst ((x,[]):xs) c = (CSPCommAction (ChanComm "mget"[ChanDotExp (ZVar ((get_proc_name x lst)++"_"++x,[])),ChanInp ("v"++(get_proc_name x lst)++"_"++x)]) (make_get_com lst xs c))
+make_get_com lst x c = c   
+
+get_proc_name :: ZName -> [(ZName, ZVar, ZExpr)] -> ZName
+get_proc_name x [(a,(va,x1),b)]
+ = case x == va of
+  True -> a
+  _ -> ""
+get_proc_name x ((a,(va,x1),b):vst)
+ = case x == va of
+  True -> a
+  _ -> get_proc_name x vst
+
+
+
+-- Defsets.hs
+
 getWrtV xs = []
 
+free_var_CAction :: CAction -> [ZVar]
+free_var_CAction (CActionCommand c) = (free_var_comnd c)
+free_var_CAction (CSPCommAction (ChanComm com xs) c) = (get_chan_param xs)++(free_var_CAction c)
+free_var_CAction (CSPGuard p c) = (free_var_ZPred p)++(free_var_CAction c)
+free_var_CAction (CSPSeq ca cb) = (free_var_CAction ca)++(free_var_CAction cb)
+free_var_CAction (CSPExtChoice ca cb) = (free_var_CAction ca)++(free_var_CAction cb)
+free_var_CAction (CSPIntChoice ca cb) = (free_var_CAction ca)++(free_var_CAction cb)
+free_var_CAction (CSPNSParal ns1 cs ns2 ca cb) = (free_var_CAction ca)++(free_var_CAction cb)
+free_var_CAction (CSPParal cs ca cb) = (free_var_CAction ca)++(free_var_CAction cb)
+free_var_CAction (CSPNSInter ns1 ns2 ca cb) = (free_var_CAction ca)++(free_var_CAction cb)
+free_var_CAction (CSPInterleave ca cb) = (free_var_CAction ca)++(free_var_CAction cb)
+free_var_CAction (CSPHide c cs) = (free_var_CAction c)
+free_var_CAction (CSPRecursion nm c) = (free_var_CAction c)
+free_var_CAction (CSPUnParAction lst c nm) = (free_var_CAction c) \\ (fvs free_var_ZGenFilt lst)
+free_var_CAction (CSPRepSeq lst c) = (free_var_CAction c) \\ (fvs free_var_ZGenFilt lst)
+free_var_CAction (CSPRepExtChoice lst c) = (free_var_CAction c) \\ (fvs free_var_ZGenFilt lst)
+free_var_CAction (CSPRepIntChoice lst c) = (free_var_CAction c) \\ (fvs free_var_ZGenFilt lst)
+free_var_CAction (CSPRepParalNS cs lst ns c) = (free_var_CAction c) \\ (fvs free_var_ZGenFilt lst)
+free_var_CAction (CSPRepParal cs lst c) = (free_var_CAction c) \\ (fvs free_var_ZGenFilt lst)
+free_var_CAction (CSPRepInterlNS lst ns c) = (free_var_CAction c) \\ (fvs free_var_ZGenFilt lst)
+free_var_CAction (CSPRepInterl lst c) = (free_var_CAction c) \\ (fvs free_var_ZGenFilt lst)
+free_var_CAction _ = []
 
+free_var_ZGenFilt (Choose v e) = [v]
+free_var_ZGenFilt _ = []
 
-getFV xs = []
+free_var_comnd (CAssign v e) = v
+free_var_comnd (CIf ga) = free_var_if ga
+free_var_comnd (CVarDecl z c) = (free_var_CAction c) \\ (fvs free_var_ZGenFilt z)
+free_var_comnd (CommandBrace z) = (free_var_ZPred z)
+free_var_comnd (CommandBracket z) = (free_var_ZPred z)
+free_var_comnd (CValDecl z c) = (free_var_CAction c) \\ (fvs free_var_ZGenFilt z)
+free_var_comnd (CResDecl z c) = (free_var_CAction c) \\ (fvs free_var_ZGenFilt z)
+free_var_comnd (CVResDecl z c) = (free_var_CAction c) \\ (fvs free_var_ZGenFilt z)
+free_var_comnd _ = []
+ 
+free_var_if (CircGAction p a) = (free_var_ZPred p)++(free_var_CAction a)
+free_var_if (CircThenElse ga gb) = (free_var_if ga)++(free_var_if gb)
+free_var_if (CircElse (CircusAction a)) = (free_var_CAction a)
+free_var_if (CircElse (ParamActionDecl x (CircusAction a))) = (free_var_CAction a) \\ (fvs free_var_ZGenFilt x)
 
-
-
-join_name n v = n ++ "_" ++ v
-
-
-
-free_var_ZExpr :: ZExpr -> [ZVar]
-
-free_var_ZExpr(ZVar v)
- = [v]
-free_var_ZExpr(ZInt c )
- = []
-free_var_ZExpr(ZGiven a)
-	= error "Don't know what free vars of ZGiven are right now. Check back later"
-
-free_var_ZExpr(ZFree0 a)
-	= error "Don't know what free vars of ZFree0 are right now. Check back later"
-
-free_var_ZExpr(ZFree1 v ex)
-	= error "Don't know what free vars of ZFree1 are right now. Check back later"
-free_var_ZExpr(ZTuple exls )
- = fvs free_var_ZExpr exls
-free_var_ZExpr(ZBinding a)
-	= error "Don't know what free vars of ZBinding are right now. Check back later"
-free_var_ZExpr(ZSetDisplay exls )
- = fvs free_var_ZExpr exls
-free_var_ZExpr(ZSeqDisplay exls )
- = fvs free_var_ZExpr exls
-free_var_ZExpr(ZFSet fs )
-	= error "Don't know what free vars of ZFSet are right now. Check back later"
-free_var_ZExpr(ZIntSet zi1 zi2)
-	= error "Don't know what free vars of ZIntSet are right now. Check back later"
-free_var_ZExpr(ZGenerator rl ex)
-	= error "Don't know what free vars of ZGenerator are right now. Check back later"
-free_var_ZExpr(ZCross exls )
- = fvs free_var_ZExpr exls
-free_var_ZExpr(ZFreeType zv zbls)
-	= error "Don't know what free vars of ZFreeType are right now. Check back later"
-free_var_ZExpr(ZPowerSet{baseset=b, is_non_empty=e, is_finite=fs})
-	= error "Don't know what free vars of ZPowerSet are right now. Check back later"
-free_var_ZExpr(ZFuncSet{domset=d, ranset=r, is_function=f, is_total=t, is_onto=o, is_one2one=oo, is_sequence=s, is_non_empty=ne, is_finite=ff})
-	= error "Don't know what free vars of ZFree0 are right now. Check back later"
-free_var_ZExpr(ZSetComp gfls ma)
-	= error "Don't know what free vars of ZSetComp are right now. Check back later"
-free_var_ZExpr(ZLambda [Choose v e] a)
- = (free_var_ZExpr a) \\ [v]
-free_var_ZExpr(ZLambda _ a)
- = []
-free_var_ZExpr(ZESchema a)
-	= error "Don't know what free vars of ZESchema are right now. Check back later"
-free_var_ZExpr(ZGivenSet a)
-	= error "Don't know what free vars of ZGivenSet are right now. Check back later"
-free_var_ZExpr(ZUniverse)
-	= error "Don't know what free vars of ZUniverse are right now. Check back later"
-free_var_ZExpr(ZCall ex ex2)
- = free_var_ZExpr ex2 -- is this right??
-free_var_ZExpr(ZReln rl )
-	= error "Don't know what free vars of ZReln are right now. Check back later"
-free_var_ZExpr(ZFunc1 a)
-	= error "Don't know what free vars of ZFunc1 are right now. Check back later"
-free_var_ZExpr(ZFunc2 a)
-	= error "Don't know what free vars of ZFunc2 are right now. Check back later"
-free_var_ZExpr(ZStrange zs )
-	= error "Don't know what free vars of ZStrange are right now. Check back later"
-free_var_ZExpr(ZMu zgls mex)
-	= error "Don't know what free vars of ZMu are right now. Check back later"
-free_var_ZExpr(ZELet ves pr)
-	= ((free_var_ZExpr(pr)) \\ (map fst ves)) ++ fvs free_var_ZExpr (map snd ves)
-free_var_ZExpr(ZIf_Then_Else zp ex ex1)
-	= error "Don't know what free vars of ZIf_Then_Else are right now. Check back later"
--- free_var_ZExpr(ZIf_Then_Else zp ex ex1)
- -- = free_var_ZPred zp ++ free_var_ZExpr ex ++ free_var_ZExpr ex1
-free_var_ZExpr(ZSelect ex zv)
-	= free_var_ZExpr ex ++ [zv] 
-free_var_ZExpr(ZTheta zsx)
-	= error "Don't know what free vars of ZTheta are right now. Check back later"
 
 free_var_ZPred :: ZPred -> [ZVar]
 free_var_ZPred (ZFalse{reason=p})
-	= error "Don't know what free vars of ZFalse are right now. Check back later"
+  = error "Don't know what free vars of ZFalse are right now. Check back later"
 free_var_ZPred (ZTrue{reason=p})
-	= error "Don't know what free vars of ZTrue are right now. Check back later"
+  = error "Don't know what free vars of ZTrue are right now. Check back later"
 free_var_ZPred (ZAnd a b)
  = free_var_ZPred a ++ free_var_ZPred b
 free_var_ZPred (ZOr a b)
@@ -112,274 +102,157 @@ free_var_ZPred (ZNot a)
 free_var_ZPred (ZExists [Choose v e] a)
  = (free_var_ZPred a) \\ [v]
 free_var_ZPred (ZExists ls a)
-	= error "Don't know what free vars of ZExists are right now. Check back later"
+  = error "Don't know what free vars of ZExists are right now. Check back later"
 free_var_ZPred (ZExists_1 [Choose v e] a)
  = (free_var_ZPred a) \\ [v]
 free_var_ZPred (ZExists_1 ls a)
-	= error "Don't know what free vars of ZExists_1 are right now. Check back later"
+  = error "Don't know what free vars of ZExists_1 are right now. Check back later"
 free_var_ZPred (ZForall [Choose v e] a)
  = (free_var_ZPred a) \\ [v]
 free_var_ZPred (ZForall ls a)
-	= error "Don't know what free vars of ZForall are right now. Check back later"
+  = error "Don't know what free vars of ZForall are right now. Check back later"
 free_var_ZPred (ZPLet ls a )
-	 = error "Don't know what free vars of ZPLet are right now. Check back later"
+   = error "Don't know what free vars of ZPLet are right now. Check back later"
 free_var_ZPred (ZEqual expa expb)
  = free_var_ZExpr expa ++ free_var_ZExpr expb
 free_var_ZPred (ZMember expa expb)
-	= free_var_ZExpr expa
+  = free_var_ZExpr expa
 free_var_ZPred (ZPre zsexpr)
-	= error "Don't know what free vars of ZPre are right now. Check back later"
+  = error "Don't know what free vars of ZPre are right now. Check back later"
 free_var_ZPred (ZPSchema zsexpr)
-	= error "Don't know what free vars of ZPSchema are right now. Check back later"
-
-
+  = error "Don't know what free vars of ZPSchema are right now. Check back later"
 
 fvs f [] = []
 fvs f (e:es)
  = f(e) ++ (fvs f (es))
 
-
-
-subset xs ys = all (`elem` ys) xs
-
-
-
-free_var_CAction :: CAction -> [ZVar]
-free_var_CAction (CActionSchemaExpr x)
- = []
-free_var_CAction (CActionCommand c)
- = (free_var_comnd c)
-free_var_CAction (CActionName nm)
- = []
-free_var_CAction (CSPSkip)
- = []
-free_var_CAction (CSPStop)
- = []
-free_var_CAction (CSPChaos)
- = []
-free_var_CAction (CSPCommAction (ChanComm com xs) c)
- = (get_chan_param xs)++(free_var_CAction c)
-free_var_CAction (CSPGuard p c)
- = (free_var_ZPred p)++(free_var_CAction c)
-free_var_CAction (CSPSeq ca cb)
- = (free_var_CAction ca)++(free_var_CAction cb)
-free_var_CAction (CSPExtChoice ca cb)
- = (free_var_CAction ca)++(free_var_CAction cb)
-free_var_CAction (CSPIntChoice ca cb)
- = (free_var_CAction ca)++(free_var_CAction cb)
-free_var_CAction (CSPNSParal ns1 cs ns2 ca cb)
- = (free_var_CAction ca)++(free_var_CAction cb)
-free_var_CAction (CSPParal cs ca cb)
- = (free_var_CAction ca)++(free_var_CAction cb)
-free_var_CAction (CSPNSInter ns1 ns2 ca cb)
- = (free_var_CAction ca)++(free_var_CAction cb)
-free_var_CAction (CSPInterleave ca cb)
- = (free_var_CAction ca)++(free_var_CAction cb)
-free_var_CAction (CSPHide c cs)
- = (free_var_CAction c)
-free_var_CAction (CSPParAction nm xp)
- = []
-free_var_CAction (CSPRenAction nm cr)
- = []
-free_var_CAction (CSPRecursion nm c)
- = (free_var_CAction c)
-free_var_CAction (CSPUnParAction lst c nm)
- = (free_var_CAction c) \\ (fvs free_var_ZGenFilt lst)
-free_var_CAction (CSPRepSeq lst c)
- = (free_var_CAction c) \\ (fvs free_var_ZGenFilt lst)
-free_var_CAction (CSPRepExtChoice lst c)
- = (free_var_CAction c) \\ (fvs free_var_ZGenFilt lst)
-free_var_CAction (CSPRepIntChoice lst c)
- = (free_var_CAction c) \\ (fvs free_var_ZGenFilt lst)
-free_var_CAction (CSPRepParalNS cs lst ns c)
- = (free_var_CAction c) \\ (fvs free_var_ZGenFilt lst)
-free_var_CAction (CSPRepParal cs lst c)
- = (free_var_CAction c) \\ (fvs free_var_ZGenFilt lst)
-free_var_CAction (CSPRepInterlNS lst ns c)
- = (free_var_CAction c) \\ (fvs free_var_ZGenFilt lst)
-free_var_CAction (CSPRepInterl lst c)
- = (free_var_CAction c) \\ (fvs free_var_ZGenFilt lst)
+free_var_ZExpr :: ZExpr -> [ZVar]
+free_var_ZExpr(ZVar v) = [v]
+free_var_ZExpr(ZInt c ) = []
+free_var_ZExpr(ZTuple exls ) = fvs free_var_ZExpr exls
+free_var_ZExpr(ZSetDisplay exls ) = fvs free_var_ZExpr exls
+free_var_ZExpr(ZSeqDisplay exls ) = fvs free_var_ZExpr exls
+free_var_ZExpr(ZCross exls ) = fvs free_var_ZExpr exls
+free_var_ZExpr(ZPowerSet{baseset=b, is_non_empty=e, is_finite=fs}) = error "Don't know what free vars of ZPowerSet are right now. Check back later"
+free_var_ZExpr(ZFuncSet{domset=d, ranset=r, is_function=f, is_total=t, is_onto=o, is_one2one=oo, is_sequence=s, is_non_empty=ne, is_finite=ff}) = error "Don't know what free vars of ZFree0 are right now. Check back later"
+free_var_ZExpr(ZLambda [Choose v e] a) = (free_var_ZExpr a) \\ [v]
+free_var_ZExpr(ZLambda _ a) = []
+free_var_ZExpr(ZCall ex ex2) = free_var_ZExpr ex2 -- is this right??
+free_var_ZExpr(ZELet ves pr) = ((free_var_ZExpr(pr)) \\ (map fst ves)) ++ fvs free_var_ZExpr (map snd ves)
+-- free_var_ZExpr(ZIf_Then_Else zp ex ex1) -- = free_var_ZPred zp ++ free_var_ZExpr ex ++ free_var_ZExpr ex1
+free_var_ZExpr(ZSelect ex zv) = free_var_ZExpr ex ++ [zv]
+free_var_ZExpr _ = []
 
 
 
-free_var_comnd (CAssign v e) 
- = v
-free_var_comnd (CIf ga) 
- = free_var_if ga
-free_var_comnd (CVarDecl z c) 
- = (free_var_CAction c) \\ (fvs free_var_ZGenFilt z)
-free_var_comnd (CAssumpt n p1 p2) 
- = []
-free_var_comnd (CAssumpt1 n p) 
- = []
-free_var_comnd (CPrefix p1 p2) 
- = []
-free_var_comnd (CPrefix1 p) 
- = []
-free_var_comnd (CommandBrace z) 
- = (free_var_ZPred z)
-free_var_comnd (CommandBracket z) 
- = (free_var_ZPred z)
-free_var_comnd (CValDecl z c) 
- = (free_var_CAction c) \\ (fvs free_var_ZGenFilt z)
-free_var_comnd (CResDecl z c) 
- = (free_var_CAction c) \\ (fvs free_var_ZGenFilt z)
-free_var_comnd (CVResDecl z c) 
- = (free_var_CAction c) \\ (fvs free_var_ZGenFilt z)
+rename_vars_CAction lst (CActionSchemaExpr zsexp) = (CActionSchemaExpr zsexp)
+rename_vars_CAction lst (CActionCommand cmd) = (CActionCommand (rename_vars_CCommand lst cmd))
+rename_vars_CAction lst (CActionName zn) = (CActionName zn)
+rename_vars_CAction lst (CSPSkip ) = (CSPSkip )
+rename_vars_CAction lst (CSPStop ) = (CSPStop )
+rename_vars_CAction lst (CSPChaos) = (CSPChaos)
+rename_vars_CAction lst (CSPCommAction c a) = (CSPCommAction (rename_vars_Comm lst c) (rename_vars_CAction lst a))
+rename_vars_CAction lst (CSPGuard zp a) = (CSPGuard (rename_ZPred lst zp) (rename_vars_CAction lst a))
+rename_vars_CAction lst (CSPSeq a1 a2) = (CSPSeq (rename_vars_CAction lst a1) (rename_vars_CAction lst a2))
+rename_vars_CAction lst (CSPExtChoice a1 a2) = (CSPExtChoice (rename_vars_CAction lst a1) (rename_vars_CAction lst a2))
+rename_vars_CAction lst (CSPIntChoice a1 a2) = (CSPIntChoice (rename_vars_CAction lst a1) (rename_vars_CAction lst a2))
+rename_vars_CAction lst (CSPNSParal ns1 cs ns2 a1 a2) = (CSPNSParal ns1 cs ns2 (rename_vars_CAction lst a1) (rename_vars_CAction lst a2))
+rename_vars_CAction lst (CSPParal cs a1 a2) = (CSPParal cs (rename_vars_CAction lst a1) (rename_vars_CAction lst a2))
+rename_vars_CAction lst (CSPNSInter ns1 ns2 a1 a2) = (CSPNSInter ns1 ns2 (rename_vars_CAction lst a1) (rename_vars_CAction lst a2))
+rename_vars_CAction lst (CSPInterleave a1 a2) = (CSPInterleave (rename_vars_CAction lst a1) (rename_vars_CAction lst a2))
+rename_vars_CAction lst (CSPHide a cs) = (CSPHide (rename_vars_CAction lst a) cs)
+rename_vars_CAction lst (CSPParAction zn zexprls) = (CSPParAction zn (map (rename_ZExpr lst) zexprls))
+rename_vars_CAction lst (CSPRenAction zn crpl) = (CSPRenAction zn (rename_vars_CReplace lst crpl))
+rename_vars_CAction lst (CSPRecursion zn a) = (CSPRecursion zn (rename_vars_CAction lst a))
+rename_vars_CAction lst (CSPUnParAction zgf a zn) = (CSPUnParAction zgf (rename_vars_CAction lst a) zn)
+rename_vars_CAction lst (CSPRepSeq zgf a) = (CSPRepSeq zgf (rename_vars_CAction lst a))
+rename_vars_CAction lst (CSPRepExtChoice zgf a) = (CSPRepExtChoice zgf (rename_vars_CAction lst a))
+rename_vars_CAction lst (CSPRepIntChoice zgf a) = (CSPRepIntChoice zgf (rename_vars_CAction lst a))
+rename_vars_CAction lst (CSPRepParalNS cs zgf ns a) = (CSPRepParalNS cs zgf ns (rename_vars_CAction lst a))
+rename_vars_CAction lst (CSPRepParal cs zgf a) = (CSPRepParal cs zgf (rename_vars_CAction lst a))
+rename_vars_CAction lst (CSPRepInterlNS zgf ns a) = (CSPRepInterlNS zgf ns (rename_vars_CAction lst a))
+rename_vars_CAction lst (CSPRepInterl zgf a) = (CSPRepInterl zgf (rename_vars_CAction lst a))
+rename_vars_CAction lst x = x
 
+rename_vars_CCommand lst (CAssign zvarls1 zexprls) = (CAssign zvarls1 (map (rename_ZExpr lst) zexprls))
+rename_vars_CCommand lst (CIf ga) = (CIf (rename_vars_CGActions lst ga))
+rename_vars_CCommand lst (CVarDecl zgf a) = (CVarDecl zgf (rename_vars_CAction lst a))
+rename_vars_CCommand lst (CAssumpt znls zp1 zp2) = (CAssumpt znls (rename_ZPred lst zp1) zp2)
+rename_vars_CCommand lst (CAssumpt1 znls zp) = (CAssumpt1 znls zp)
+rename_vars_CCommand lst (CPrefix zp1 zp2) = (CPrefix (rename_ZPred lst zp1) zp2)
+rename_vars_CCommand lst (CPrefix1 zp) = (CPrefix1 zp)
+rename_vars_CCommand lst (CommandBrace zp) = (CommandBrace zp)
+rename_vars_CCommand lst (CommandBracket zp) = (CommandBracket zp)
+rename_vars_CCommand lst (CValDecl zgf a) = (CValDecl zgf (rename_vars_CAction lst a))
+rename_vars_CCommand lst (CResDecl zgf a) = (CResDecl zgf (rename_vars_CAction lst a))
+rename_vars_CCommand lst (CVResDecl zgf a) = (CVResDecl zgf (rename_vars_CAction lst a))
 
+rename_vars_CReplace lst (CRename zvarls1 zvarls) = (CRename zvarls1 zvarls)
+rename_vars_CReplace lst (CRenameAssign zvarls1 zvarls) = (CRenameAssign zvarls1 zvarls)
 
-free_var_ZGenFilt (Include s) = []
-free_var_ZGenFilt (Choose v e) = [v]
-free_var_ZGenFilt (Check p) = []
-free_var_ZGenFilt (Evaluate v e1 e2) = []
+rename_vars_Comm lst (ChanComm zn cpls) = (ChanComm zn (map (rename_vars_CParameter lst) cpls))
+rename_vars_Comm lst (ChanGenComm zn zexprls cpls) = (ChanGenComm zn (map (rename_ZExpr lst) zexprls) (map (rename_vars_CParameter lst) cpls))
 
+rename_vars_CParameter lst (ChanInp zn) = (ChanInp zn)
+rename_vars_CParameter lst (ChanInpPred zn zp) = (ChanInpPred zn (rename_ZPred lst zp))
+rename_vars_CParameter lst (ChanOutExp ze) = (ChanOutExp (rename_ZExpr lst ze))
+rename_vars_CParameter lst (ChanDotExp ze) = (ChanDotExp (rename_ZExpr lst ze))
 
+rename_vars_CGActions lst (CircGAction zp a) = (CircGAction (rename_ZPred lst zp) (rename_vars_CAction lst a))
+rename_vars_CGActions lst (CircThenElse cga1 cga2) = (CircThenElse (rename_vars_CGActions lst cga1) (rename_vars_CGActions lst cga2))
+rename_vars_CGActions lst (CircElse pa) = (CircElse pa)
 
-free_var_if (CircGAction p a)
- = (free_var_ZPred p)++(free_var_CAction a)
-free_var_if (CircThenElse ga gb)
- = (free_var_if ga)++(free_var_if gb)
-free_var_if (CircElse (CircusAction a))
- = (free_var_CAction a)
-free_var_if (CircElse (ParamActionDecl x (CircusAction a)))
- = (free_var_CAction a) \\ (fvs free_var_ZGenFilt x)
+rename_ZExpr lst (ZVar (va,x))
+ = case (inListVar va lst) of
+   True -> (ZVar ("v_"++va,x))
+   False -> (ZVar (va,x))
+rename_ZExpr lst (ZInt zi) = (ZInt zi)
+rename_ZExpr lst (ZGiven gv) = (ZGiven gv)
+rename_ZExpr lst (ZFree0 va) = (ZFree0 va)
+rename_ZExpr lst (ZFree1 va xpr) = (ZFree1 va (rename_ZExpr lst xpr))
+rename_ZExpr lst (ZTuple xprlst) = (ZTuple (map (rename_ZExpr lst) xprlst))
+rename_ZExpr lst (ZBinding xs) = (ZBinding (bindingsVar lst xs))
+rename_ZExpr lst (ZSetDisplay xprlst) = (ZSetDisplay (map (rename_ZExpr lst) xprlst))
+rename_ZExpr lst (ZSeqDisplay xprlst) = (ZSeqDisplay (map (rename_ZExpr lst) xprlst))
+rename_ZExpr lst (ZFSet zf) = (ZFSet zf)
+rename_ZExpr lst (ZIntSet i1 i2) = (ZIntSet i1 i2)
+rename_ZExpr lst (ZGenerator zrl xpr) = (ZGenerator zrl (rename_ZExpr lst xpr))
+rename_ZExpr lst (ZCross xprlst) = (ZCross (map (rename_ZExpr lst) xprlst))
+rename_ZExpr lst (ZFreeType va lst1) = (ZFreeType va lst1)
+rename_ZExpr lst (ZPowerSet{baseset=xpr, is_non_empty=b1, is_finite=b2}) = (ZPowerSet{baseset=(rename_ZExpr lst xpr), is_non_empty=b1, is_finite=b2})
+rename_ZExpr lst (ZFuncSet{ domset=expr1, ranset=expr2, is_function=b1, is_total=b2, is_onto=b3, is_one2one=b4, is_sequence=b5, is_non_empty=b6, is_finite=b7}) = (ZFuncSet{ domset=(rename_ZExpr lst expr1), ranset=(rename_ZExpr lst expr2), is_function=b1, is_total=b2, is_onto=b3, is_one2one=b4, is_sequence=b5, is_non_empty=b6, is_finite=b7})
+rename_ZExpr lst (ZSetComp lst1 (Just xpr)) = (ZSetComp lst1 (Just (rename_ZExpr lst xpr)))
+rename_ZExpr lst (ZSetComp lst1 Nothing) = (ZSetComp lst1 Nothing)
+rename_ZExpr lst (ZLambda lst1 xpr) = (ZLambda lst1 (rename_ZExpr lst xpr))
+rename_ZExpr lst (ZESchema zxp) = (ZESchema zxp)
+rename_ZExpr lst (ZGivenSet gs) = (ZGivenSet gs)
+rename_ZExpr lst (ZUniverse) = (ZUniverse)
+rename_ZExpr lst (ZCall xpr1 xpr2) = (ZCall (rename_ZExpr lst xpr1) (rename_ZExpr lst xpr2))
+rename_ZExpr lst (ZReln rl) = (ZReln rl)
+rename_ZExpr lst (ZFunc1 f1) = (ZFunc1 f1)
+rename_ZExpr lst (ZFunc2 f2) = (ZFunc2 f2)
+rename_ZExpr lst (ZStrange st) = (ZStrange st)
+rename_ZExpr lst (ZMu lst1 (Just xpr)) = (ZMu lst1 (Just (rename_ZExpr lst xpr)))
+rename_ZExpr lst (ZELet lst1 xpr1) = (ZELet (bindingsVar lst lst1) (rename_ZExpr lst xpr1))
+rename_ZExpr lst (ZIf_Then_Else zp xpr1 xpr2) = (ZIf_Then_Else zp (rename_ZExpr lst xpr1) (rename_ZExpr lst xpr2))
+rename_ZExpr lst (ZSelect xpr va) = (ZSelect xpr va)
+rename_ZExpr lst (ZTheta zs) = (ZTheta zs)
 
-
-   
-get_main_action :: [PPar] -> CAction -> CAction
-get_main_action lst (CActionSchemaExpr x)
- = (CActionSchemaExpr x)
-get_main_action lst (CActionCommand c)
- = (CActionCommand (get_main_action_comnd lst c))
-get_main_action lst (CActionName nm)
- = get_action nm lst
-get_main_action lst (CSPSkip)
- = (CSPSkip)
-get_main_action lst (CSPStop)
- = (CSPStop)
-get_main_action lst (CSPChaos)
- = (CSPChaos)
-get_main_action lst (CSPCommAction com c)
- = (CSPCommAction com (get_main_action lst c))
-get_main_action lst (CSPGuard p c)
- = (CSPGuard p (get_main_action lst c))
-get_main_action lst (CSPSeq ca cb)
- = (CSPSeq (get_main_action lst ca) (get_main_action lst cb))
-get_main_action lst (CSPExtChoice ca cb)
- = (CSPExtChoice (get_main_action lst ca) (get_main_action lst cb))
-get_main_action lst (CSPIntChoice ca cb)
- = (CSPIntChoice (get_main_action lst ca) (get_main_action lst cb))
-get_main_action lst (CSPNSParal ns1 cs ns2 ca cb)
- = (CSPNSParal ns1 cs ns2 (get_main_action lst ca) (get_main_action lst cb))
-get_main_action lst (CSPParal cs ca cb)
- = (CSPParal cs (get_main_action lst ca) (get_main_action lst cb))
-get_main_action lst (CSPNSInter ns1 ns2 ca cb)
- = (CSPNSInter ns1 ns2 (get_main_action lst ca) (get_main_action lst cb))
-get_main_action lst (CSPInterleave ca cb)
- = (CSPInterleave (get_main_action lst ca) (get_main_action lst cb))
-get_main_action lst (CSPHide c cs)
- = (CSPHide (get_main_action lst c) cs)
-get_main_action lst (CSPParAction nm xp)
- = (CSPParAction nm xp)
-get_main_action lst (CSPRenAction nm cr)
- = (CSPRenAction nm cr)
-get_main_action lst (CSPRecursion n (CSPSeq c (CActionName n1)))
- = case n == n1 of
-   True -> (CSPRecursion n (CSPSeq (get_main_action lst c) (CActionName n)))
-   False -> (CSPRecursion n (CSPSeq (get_main_action lst c) (CActionName n1)))
-get_main_action lst (CSPUnParAction lsta c nm)
- = (CSPUnParAction lsta (get_main_action lst c) nm)
-get_main_action lst (CSPRepSeq lsta c)
- = (CSPRepSeq lsta (get_main_action lst c))
-get_main_action lst (CSPRepExtChoice lsta c)
- = (CSPRepExtChoice lsta (get_main_action lst c))
-get_main_action lst (CSPRepIntChoice lsta c)
- = (CSPRepIntChoice lsta (get_main_action lst c))
-get_main_action lst (CSPRepParalNS cs lsta ns c)
- = (CSPRepParalNS cs lsta ns (get_main_action lst c))
-get_main_action lst (CSPRepParal cs lsta c)
- = (CSPRepParal cs lsta (get_main_action lst c))
-get_main_action lst (CSPRepInterlNS lsta ns c)
- = (CSPRepInterlNS lsta ns (get_main_action lst c))
-get_main_action lst (CSPRepInterl lsta c)
- = (CSPRepInterl lsta (get_main_action lst c))
-
-
-
-get_main_action_comnd lst (CAssign v e) 
- = (CAssign v e)
-get_main_action_comnd lst (CIf ga) 
- = (CIf (get_if lst ga))
-get_main_action_comnd lst (CVarDecl z a) 
- = (CVarDecl z (get_main_action lst a))
-get_main_action_comnd lst (CAssumpt n p1 p2) 
- = (CAssumpt n p1 p2)
-get_main_action_comnd lst (CAssumpt1 n p) 
- = (CAssumpt1 n p)
-get_main_action_comnd lst (CPrefix p1 p2) 
- = (CPrefix p1 p2)
-get_main_action_comnd lst (CPrefix1 p) 
- = (CPrefix1 p)
-get_main_action_comnd lst (CommandBrace p) 
- = (CommandBrace p)
-get_main_action_comnd lst (CommandBracket p) 
- = (CommandBracket p)
-get_main_action_comnd lst (CValDecl z a) 
- = (CValDecl z (get_main_action lst a))
-get_main_action_comnd lst (CResDecl z a) 
- = (CResDecl z (get_main_action lst a))
-get_main_action_comnd lst (CVResDecl z a) 
- = (CVResDecl z (get_main_action lst a))
-
-
-
-get_if lst (CircGAction p a)
- = (CircGAction p (get_main_action lst a))
-get_if lst (CircThenElse ga gb)
- = (CircThenElse (get_if lst ga) (get_if lst gb))
-get_if lst (CircElse (CircusAction a))
- = (CircElse (CircusAction (get_main_action lst a)))
-get_if lst (CircElse (ParamActionDecl x (CircusAction a)))
- = (CircElse (ParamActionDecl x (CircusAction (get_main_action lst a))))
-
-
-
-get_action _ [] = error "Action list is empty" 
-get_action name [(CParAction n (CircusAction a))] 
- = case name == n of
-   True -> a
-   False -> error "Action not found"
-
-get_action name ((CParAction n (CircusAction a)):xs)
- = case name == n of
-   True -> a
-   False -> get_action name xs
-
-
-
-get_chan_param :: [CParameter] -> [ZVar]
-get_chan_param [] = [] 
-get_chan_param [ChanDotExp (ZVar (x,_))] 
- = [(x,[])]
-get_chan_param [ChanOutExp (ZVar (x,_))] 
- = [(x,[])]
-get_chan_param [_] 
- = []
-get_chan_param ((ChanDotExp (ZVar (x,_))):xs) 
- = [(x,[])]++(get_chan_param xs)
-get_chan_param ((ChanOutExp (ZVar (x,_))):xs) 
- = [(x,[])]++(get_chan_param xs)
-get_chan_param (_:xs) = (get_chan_param xs)
-
-
-
-filter_state_comp :: [(ZName, ZVar, ZExpr)] -> [ZVar]
-filter_state_comp [] = []
-filter_state_comp [(_, v, _)] = [v]
-filter_state_comp ((_, v, _):xs) = [v]++(filter_state_comp xs)
-
-
+rename_ZPred lst (ZFalse{reason=a}) = (ZFalse{reason=a})
+rename_ZPred lst (ZTrue{reason=a}) = (ZTrue{reason=a})
+rename_ZPred lst (ZAnd p1 p2) = (ZAnd (rename_ZPred lst p1) (rename_ZPred lst p2))
+rename_ZPred lst (ZOr p1 p2) = (ZOr (rename_ZPred lst p1) (rename_ZPred lst p2))
+rename_ZPred lst (ZImplies p1 p2) = (ZImplies (rename_ZPred lst p1) (rename_ZPred lst p2))
+rename_ZPred lst (ZIff p1 p2) = (ZIff (rename_ZPred lst p1) (rename_ZPred lst p2))
+rename_ZPred lst (ZNot p) = (ZNot (rename_ZPred lst p))
+rename_ZPred lst (ZExists lst1 p) = (ZExists lst1 (rename_ZPred lst p))
+rename_ZPred lst (ZExists_1 lst1 p) = (ZExists_1 lst1 (rename_ZPred lst p))
+rename_ZPred lst (ZForall lst1 p) = (ZForall lst1 (rename_ZPred lst p))
+rename_ZPred lst (ZPLet varxp p) = (ZPLet varxp (rename_ZPred lst p))
+rename_ZPred lst (ZEqual xpr1 xpr2) = (ZEqual (rename_ZExpr lst xpr1) (rename_ZExpr lst xpr2))
+rename_ZPred lst (ZMember xpr1 xpr2) = (ZMember (rename_ZExpr lst xpr1) (rename_ZExpr lst xpr2))
+rename_ZPred lst (ZPre sp) = (ZPre sp)
+rename_ZPred lst (ZPSchema sp) = (ZPSchema sp)
 
 inListVar x []
  = False
@@ -391,8 +264,6 @@ inListVar x (va:vst)
  = case x == va of
   True -> True
   _ -> inListVar x vst
-
-
 
 
 bindingsVar lst []
@@ -407,682 +278,49 @@ bindingsVar lst (((va,x),b):xs)
    False -> [((va,x),(rename_ZExpr lst b))]++(bindingsVar lst xs)
 
 
+get_chan_param :: [CParameter] -> [ZVar]
+get_chan_param [] = [] 
+get_chan_param [ChanDotExp (ZVar (x,_))] = [(x,[])]
+get_chan_param [ChanOutExp (ZVar (x,_))] = [(x,[])]
+get_chan_param [_] = []
+get_chan_param ((ChanDotExp (ZVar (x,_))):xs) = [(x,[])]++(get_chan_param xs)
+get_chan_param ((ChanOutExp (ZVar (x,_))):xs) = [(x,[])]++(get_chan_param xs)
+get_chan_param (_:xs) = (get_chan_param xs)
+
+-- | The '\\' function is list difference ((non-associative).
+-- In the result of @xs@ '\\' @ys@, the first occurrence of each element of
+-- @ys@ in turn (if any) has been removed from @xs@.  Thus
+--
+-- > (xs ++ ys) \\ xs == ys.
+--
+-- It is a special case of 'deleteFirstsBy', which allows the programmer
+-- to supply their own equality test.
+
+(\\)                    :: (Eq a) => [a] -> [a] -> [a]
+(\\)                    =  foldl (flip delete)
+
+
+-- | 'delete' @x@ removes the first occurrence of @x@ from its list argument.
+-- For example,
+--
+-- > delete 'a' "banana" == "bnana"
+--
+-- It is a special case of 'deleteBy', which allows the programmer to
+-- supply their own equality test.
+
+delete                  :: (Eq a) => a -> [a] -> [a]
+delete                  =  deleteBy (==)
+
+-- | The 'deleteBy' function behaves like 'delete', but takes a
+-- user-supplied equality predicate.
+deleteBy                :: (a -> a -> Bool) -> a -> [a] -> [a]
+deleteBy _  _ []        = []
+deleteBy eq x (y:ys)    = if x `eq` y then ys else y : deleteBy eq x ys
+
+
+flip         :: (a -> b -> c) -> b -> a -> c
+flip f x y   =  f y x
 
-
-rename_ZVar lst (va,x)
-  = case (inListVar va lst) of
-     True -> ("v_"++va,x)
-     False -> (va,x)
-rename_ZExpr lst (ZVar (va,x))
- = case (inListVar va lst) of
-   True -> (ZVar ("v_"++va,x))
-   False -> (ZVar (va,x))
-rename_ZExpr lst (ZInt zi)
- = (ZInt zi)
-rename_ZExpr lst (ZGiven gv)
- = (ZGiven gv)
-rename_ZExpr lst (ZFree0 va)
- = (ZFree0 va)
-rename_ZExpr lst (ZFree1 va xpr)
- = (ZFree1 va (rename_ZExpr lst xpr))
-rename_ZExpr lst (ZTuple xprlst)
- = (ZTuple (map (rename_ZExpr lst) xprlst))
-rename_ZExpr lst (ZBinding xs)
- = (ZBinding (bindingsVar lst xs))
-rename_ZExpr lst (ZSetDisplay xprlst)
- = (ZSetDisplay (map (rename_ZExpr lst) xprlst))
-rename_ZExpr lst (ZSeqDisplay xprlst)
- = (ZSeqDisplay (map (rename_ZExpr lst) xprlst))
-rename_ZExpr lst (ZFSet zf)
- = (ZFSet zf)
-rename_ZExpr lst (ZIntSet i1 i2)
- = (ZIntSet i1 i2)
-rename_ZExpr lst (ZGenerator zrl xpr)
- = (ZGenerator zrl (rename_ZExpr lst xpr))
-rename_ZExpr lst (ZCross xprlst)
- = (ZCross (map (rename_ZExpr lst) xprlst))
-rename_ZExpr lst (ZFreeType va lst1)
- = (ZFreeType va lst1)
-rename_ZExpr lst (ZPowerSet{baseset=xpr, is_non_empty=b1, is_finite=b2})
- = (ZPowerSet{baseset=(rename_ZExpr lst xpr), is_non_empty=b1, is_finite=b2})
-rename_ZExpr lst (ZFuncSet{ domset=expr1, ranset=expr2, is_function=b1, is_total=b2, is_onto=b3, is_one2one=b4, is_sequence=b5, is_non_empty=b6, is_finite=b7})
- = (ZFuncSet{ domset=(rename_ZExpr lst expr1), ranset=(rename_ZExpr lst expr2), is_function=b1, is_total=b2, is_onto=b3, is_one2one=b4, is_sequence=b5, is_non_empty=b6, is_finite=b7})
-rename_ZExpr lst (ZSetComp lst1 (Just xpr)) 
- = (ZSetComp lst1 (Just (rename_ZExpr lst xpr)))
-rename_ZExpr lst (ZSetComp lst1 Nothing) 
- = (ZSetComp lst1 Nothing)
-rename_ZExpr lst (ZLambda lst1 xpr)
- = (ZLambda lst1 (rename_ZExpr lst xpr))
-rename_ZExpr lst (ZESchema zxp)
- = (ZESchema zxp)
-rename_ZExpr lst (ZGivenSet gs)
- = (ZGivenSet gs)
-rename_ZExpr lst (ZUniverse)
- = (ZUniverse)
-rename_ZExpr lst (ZCall xpr1 xpr2)
- = (ZCall (rename_ZExpr lst xpr1) (rename_ZExpr lst xpr2))
-rename_ZExpr lst (ZReln rl)
- = (ZReln rl)
-rename_ZExpr lst (ZFunc1 f1)
- = (ZFunc1 f1)
-rename_ZExpr lst (ZFunc2 f2)
- = (ZFunc2 f2)
-rename_ZExpr lst (ZStrange st)
- = (ZStrange st)
-rename_ZExpr lst (ZMu lst1 (Just xpr))
- = (ZMu lst1 (Just (rename_ZExpr lst xpr)))
-rename_ZExpr lst (ZELet lst1 xpr1)
- = (ZELet (bindingsVar lst lst1) (rename_ZExpr lst xpr1))
-rename_ZExpr lst (ZIf_Then_Else zp xpr1 xpr2)
- = (ZIf_Then_Else zp (rename_ZExpr lst xpr1) (rename_ZExpr lst xpr2))
-rename_ZExpr lst (ZSelect xpr va)
- = (ZSelect xpr va)
-rename_ZExpr lst (ZTheta zs)
- = (ZTheta zs)
-
-
-
-rename_ZPred lst (ZFalse{reason=a})
- = (ZFalse{reason=a})
-rename_ZPred lst (ZTrue{reason=a})
- = (ZTrue{reason=a})
-rename_ZPred lst (ZAnd p1 p2)
- = (ZAnd (rename_ZPred lst p1) (rename_ZPred lst p2))
-rename_ZPred lst (ZOr p1 p2)
- = (ZOr (rename_ZPred lst p1) (rename_ZPred lst p2))
-rename_ZPred lst (ZImplies p1 p2)
- = (ZImplies (rename_ZPred lst p1) (rename_ZPred lst p2))
-rename_ZPred lst (ZIff p1 p2)
- = (ZIff (rename_ZPred lst p1) (rename_ZPred lst p2))
-rename_ZPred lst (ZNot p)
- = (ZNot (rename_ZPred lst p))
-rename_ZPred lst (ZExists lst1 p)
- = (ZExists lst1 (rename_ZPred lst p))
-rename_ZPred lst (ZExists_1 lst1 p)
- = (ZExists_1 lst1 (rename_ZPred lst p))
-rename_ZPred lst (ZForall lst1 p)
- = (ZForall lst1 (rename_ZPred lst p))
-rename_ZPred lst (ZPLet varxp p)
- = (ZPLet varxp (rename_ZPred lst p))
-rename_ZPred lst (ZEqual xpr1 xpr2)
- = (ZEqual (rename_ZExpr lst xpr1) (rename_ZExpr lst xpr2))
-rename_ZPred lst (ZMember xpr1 xpr2)
- = (ZMember (rename_ZExpr lst xpr1) (rename_ZExpr lst xpr2))
-rename_ZPred lst (ZPre sp)
- = (ZPre sp)
-rename_ZPred lst (ZPSchema sp)
- = (ZPSchema sp)
-
-
-
-middle (a,b,c) = b
-
-
-
-rename_vars_ParAction lst (CircusAction ca) 
-  = (CircusAction (rename_vars_CAction lst ca))
-rename_vars_ParAction lst (ParamActionDecl zglst pa)
-  = (ParamActionDecl zglst (rename_vars_ParAction lst pa))
-
-
-
-rename_vars_CAction lst (CActionSchemaExpr zsexp)
- = (CActionSchemaExpr zsexp)
-rename_vars_CAction lst (CActionCommand cmd)
- = (CActionCommand (rename_vars_CCommand lst cmd))
-rename_vars_CAction lst (CActionName zn)
- = (CActionName zn)
-rename_vars_CAction lst (CSPSkip )
- = (CSPSkip )
-rename_vars_CAction lst (CSPStop )
- = (CSPStop )
-rename_vars_CAction lst (CSPChaos)
- = (CSPChaos)
-rename_vars_CAction lst (CSPCommAction c a)
- = (CSPCommAction (rename_vars_Comm lst c) (rename_vars_CAction lst a))
-rename_vars_CAction lst (CSPGuard zp a)
- = (CSPGuard (rename_ZPred lst zp) (rename_vars_CAction lst a))
-rename_vars_CAction lst (CSPSeq a1 a2)
- = (CSPSeq (rename_vars_CAction lst a1) (rename_vars_CAction lst a2))
-rename_vars_CAction lst (CSPExtChoice a1 a2)
- = (CSPExtChoice (rename_vars_CAction lst a1) (rename_vars_CAction lst a2))
-rename_vars_CAction lst (CSPIntChoice a1 a2)
- = (CSPIntChoice (rename_vars_CAction lst a1) (rename_vars_CAction lst a2))
-rename_vars_CAction lst (CSPNSParal ns1 cs ns2 a1 a2)
- = (CSPNSParal ns1 cs ns2 (rename_vars_CAction lst a1) (rename_vars_CAction lst a2))
-rename_vars_CAction lst (CSPParal cs a1 a2)
- = (CSPParal cs (rename_vars_CAction lst a1) (rename_vars_CAction lst a2))
-rename_vars_CAction lst (CSPNSInter ns1 ns2 a1 a2)
- = (CSPNSInter ns1 ns2 (rename_vars_CAction lst a1) (rename_vars_CAction lst a2))
-rename_vars_CAction lst (CSPInterleave a1 a2)
- = (CSPInterleave (rename_vars_CAction lst a1) (rename_vars_CAction lst a2))
-rename_vars_CAction lst (CSPHide a cs)
- = (CSPHide (rename_vars_CAction lst a) cs)
-rename_vars_CAction lst (CSPParAction zn zexprls)
- = (CSPParAction zn (map (rename_ZExpr lst) zexprls))
-rename_vars_CAction lst (CSPRenAction zn crpl)
- = (CSPRenAction zn (rename_vars_CReplace lst crpl))
-rename_vars_CAction lst (CSPRecursion zn a)
- = (CSPRecursion zn (rename_vars_CAction lst a))
-rename_vars_CAction lst (CSPUnParAction zgf a zn)
- = (CSPUnParAction zgf (rename_vars_CAction lst a) zn)
-rename_vars_CAction lst (CSPRepSeq zgf a)
- = (CSPRepSeq zgf (rename_vars_CAction lst a))
-rename_vars_CAction lst (CSPRepExtChoice zgf a)
- = (CSPRepExtChoice zgf (rename_vars_CAction lst a))
-rename_vars_CAction lst (CSPRepIntChoice zgf a)
- = (CSPRepIntChoice zgf (rename_vars_CAction lst a))
-rename_vars_CAction lst (CSPRepParalNS cs zgf ns a)
- = (CSPRepParalNS cs zgf ns (rename_vars_CAction lst a))
-rename_vars_CAction lst (CSPRepParal cs zgf a)
- = (CSPRepParal cs zgf (rename_vars_CAction lst a))
-rename_vars_CAction lst (CSPRepInterlNS zgf ns a)
- = (CSPRepInterlNS zgf ns (rename_vars_CAction lst a))
-rename_vars_CAction lst (CSPRepInterl zgf a)
- = (CSPRepInterl zgf (rename_vars_CAction lst a))
-
-
-
-rename_vars_Comm lst (ChanComm zn cpls)
- = (ChanComm zn (map (rename_vars_CParameter lst) cpls))
-rename_vars_Comm lst (ChanGenComm zn zexprls cpls)
- = (ChanGenComm zn (map (rename_ZExpr lst) zexprls) (map (rename_vars_CParameter lst) cpls))
-
-
-
-rename_vars_CParameter lst (ChanInp zn)
- = (ChanInp zn)
-rename_vars_CParameter lst (ChanInpPred zn zp)
- = (ChanInpPred zn (rename_ZPred lst zp))
-rename_vars_CParameter lst (ChanOutExp ze)
- = (ChanOutExp (rename_ZExpr lst ze))
-rename_vars_CParameter lst (ChanDotExp ze)
- = (ChanDotExp (rename_ZExpr lst ze))
-
-
-
-rename_vars_CCommand lst (CAssign zvarls1 zexprls)
- = (CAssign zvarls1 (map (rename_ZExpr lst) zexprls))
-rename_vars_CCommand lst (CIf ga)
- = (CIf (rename_vars_CGActions lst ga))
-rename_vars_CCommand lst (CVarDecl zgf a)
- = (CVarDecl zgf (rename_vars_CAction lst a))
-rename_vars_CCommand lst (CAssumpt znls zp1 zp2)
- = (CAssumpt znls (rename_ZPred lst zp1) zp2)
-rename_vars_CCommand lst (CAssumpt1 znls zp)
- = (CAssumpt1 znls zp)
-rename_vars_CCommand lst (CPrefix zp1 zp2)
- = (CPrefix (rename_ZPred lst zp1) zp2)
-rename_vars_CCommand lst (CPrefix1 zp)
- = (CPrefix1 zp)
-rename_vars_CCommand lst (CommandBrace zp)
- = (CommandBrace zp)
-rename_vars_CCommand lst (CommandBracket zp)
- = (CommandBracket zp)
-rename_vars_CCommand lst (CValDecl zgf a)
- = (CValDecl zgf (rename_vars_CAction lst a))
-rename_vars_CCommand lst (CResDecl zgf a)
- = (CResDecl zgf (rename_vars_CAction lst a))
-rename_vars_CCommand lst (CVResDecl zgf a)
- = (CVResDecl zgf (rename_vars_CAction lst a))
-
-
-
-rename_vars_CGActions lst (CircGAction zp a)
- = (CircGAction (rename_ZPred lst zp) (rename_vars_CAction lst a))
-rename_vars_CGActions lst (CircThenElse cga1 cga2)
- = (CircThenElse (rename_vars_CGActions lst cga1) (rename_vars_CGActions lst cga2))
-rename_vars_CGActions lst (CircElse pa)
- = (CircElse pa)
-
-
-
-rename_vars_CReplace lst (CRename zvarls1 zvarls)
- = (CRename zvarls1 zvarls)
-rename_vars_CReplace lst (CRenameAssign zvarls1 zvarls)
- = (CRenameAssign zvarls1 zvarls)
-
-
-
-rename_vars_ZPara1 :: [(ZName, ZVar, ZExpr)] -> ZPara -> ZPara
-rename_vars_ZPara1 lst (Process zp)
-  = (Process (rename_vars_ProcDecl1 lst zp))
-rename_vars_ZPara1 lst x 
-  = x 
-
-
-
-rename_vars_ProcDecl1 :: [(ZName, ZVar, ZExpr)] -> ProcDecl -> ProcDecl
-rename_vars_ProcDecl1 lst (CProcess zn pd)
-  = (CProcess zn (rename_vars_ProcessDef1 lst pd))
-rename_vars_ProcDecl1 lst (CParamProcess zn znls pd)
-  = (CParamProcess zn znls (rename_vars_ProcessDef1 lst pd))
-rename_vars_ProcDecl1 lst (CGenProcess zn znls pd)
-  = (CParamProcess zn znls (rename_vars_ProcessDef1 lst pd))
-
-
-
-rename_vars_ProcessDef1 :: [(ZName, ZVar, ZExpr)] -> ProcessDef -> ProcessDef
-rename_vars_ProcessDef1 lst (ProcDefSpot zgf pd)
-  = (ProcDefSpot zgf (rename_vars_ProcessDef1 lst pd))
-rename_vars_ProcessDef1 lst (ProcDefIndex zgf pd)
-  = (ProcDefIndex zgf (rename_vars_ProcessDef1 lst pd))
-rename_vars_ProcessDef1 lst (ProcDef cp)
-  = (ProcDef (rename_vars_CProc1 lst cp))
-
-
-
-rename_vars_CProc1 :: [(ZName, ZVar, ZExpr)] -> CProc -> CProc
-rename_vars_CProc1 lst (CRepSeqProc zgf cp)
-  = (CRepSeqProc zgf (rename_vars_CProc1 lst cp))
-rename_vars_CProc1 lst (CRepExtChProc zgf cp)
-  = (CRepExtChProc zgf (rename_vars_CProc1 lst cp))
-rename_vars_CProc1 lst (CRepIntChProc zgf cp)
-  = (CRepIntChProc zgf (rename_vars_CProc1 lst cp))
-rename_vars_CProc1 lst (CRepParalProc cs zgf cp)
-  = (CRepParalProc cs zgf (rename_vars_CProc1 lst cp))
-rename_vars_CProc1 lst (CRepInterlProc zgf cp)
-  = (CRepInterlProc zgf (rename_vars_CProc1 lst cp))
-rename_vars_CProc1 lst (CHide cp cxp)
-  = (CHide (rename_vars_CProc1 lst cp) cxp)
-rename_vars_CProc1 lst (CExtChoice cp1 cp2)
-  = (CExtChoice (rename_vars_CProc1 lst cp1) (rename_vars_CProc1 lst cp2))
-rename_vars_CProc1 lst (CIntChoice cp1 cp2)
-  = (CIntChoice (rename_vars_CProc1 lst cp1) (rename_vars_CProc1 lst cp2))
-rename_vars_CProc1 lst (CParParal cs cp1 cp2)
-  = (CParParal cs (rename_vars_CProc1 lst cp1) (rename_vars_CProc1 lst cp2))
-rename_vars_CProc1 lst (CInterleave cp1 cp2)
-  = (CInterleave (rename_vars_CProc1 lst cp1) (rename_vars_CProc1 lst cp2))
-rename_vars_CProc1 lst (CGenProc zn zxp)
-  = (CGenProc zn zxp)
-rename_vars_CProc1 lst (CParamProc zn zxp)
-  = (CParamProc zn zxp)
-rename_vars_CProc1 lst (CProcRename zn c1 c2)
-  = (CProcRename zn c1 c2)
-rename_vars_CProc1 lst (CSeq cp1 cp2)
-  = (CSeq (rename_vars_CProc1 lst cp1) (rename_vars_CProc1 lst cp2))
-rename_vars_CProc1 lst (CSimpIndexProc zn zxp)
-  = (CSimpIndexProc zn zxp)
-rename_vars_CProc1 lst (CircusProc zn)
-  = (CircusProc zn)
-rename_vars_CProc1 lst (ProcMain zp ppl ca)
-  = (ProcMain zp (map (rename_vars_PPar1 lst) ppl) (rename_vars_CAction1 lst ca))
-rename_vars_CProc1 lst (ProcStalessMain ppl ca)
-  = (ProcStalessMain ppl (rename_vars_CAction1 lst ca))
-
-
-
-rename_vars_PPar1 :: [(ZName, ZVar, ZExpr)] -> PPar -> PPar
-rename_vars_PPar1 lst (ProcZPara zp) 
-  = (ProcZPara zp)
-rename_vars_PPar1 lst (CParAction zn pa) 
-  = (CParAction zn (rename_vars_ParAction1 lst pa))
-rename_vars_PPar1 lst (CNameSet zn ns) 
-  = (CNameSet zn ns)
-
-
-
-rename_vars_ParAction1 :: [(ZName, ZVar, ZExpr)] -> ParAction -> ParAction
-rename_vars_ParAction1 lst (CircusAction ca) 
-  = (CircusAction (rename_vars_CAction1 lst ca))
-rename_vars_ParAction1 lst (ParamActionDecl zgf pa) 
-  = (ParamActionDecl zgf (rename_vars_ParAction1 lst pa))
-
-
-
-rename_vars_CAction1 :: [(ZName, ZVar, ZExpr)] -> CAction -> CAction
-rename_vars_CAction1 lst (CActionSchemaExpr zsexp)
- = (CActionSchemaExpr zsexp)
-rename_vars_CAction1 lst (CActionCommand cmd)
- = (CActionCommand (rename_vars_CCommand1 lst cmd))
-rename_vars_CAction1 lst (CActionName zn)
- = (CActionName zn)
-rename_vars_CAction1 lst (CSPSkip )
- = (CSPSkip )
-rename_vars_CAction1 lst (CSPStop )
- = (CSPStop )
-rename_vars_CAction1 lst (CSPChaos)
- = (CSPChaos)
-rename_vars_CAction1 lst (CSPCommAction c a)
- = (CSPCommAction (rename_vars_Comm1 lst c) (rename_vars_CAction1 lst a))
-rename_vars_CAction1 lst (CSPGuard zp a)
- = (CSPGuard (rename_vars_ZPred1 lst zp) (rename_vars_CAction1 lst a))
-rename_vars_CAction1 lst (CSPSeq a1 a2)
- = (CSPSeq (rename_vars_CAction1 lst a1) (rename_vars_CAction1 lst a2))
-rename_vars_CAction1 lst (CSPExtChoice a1 a2)
- = (CSPExtChoice (rename_vars_CAction1 lst a1) (rename_vars_CAction1 lst a2))
-rename_vars_CAction1 lst (CSPIntChoice a1 a2)
- = (CSPIntChoice (rename_vars_CAction1 lst a1) (rename_vars_CAction1 lst a2))
-rename_vars_CAction1 lst (CSPNSParal ns1 cs ns2 a1 a2)
- = (CSPNSParal ns1 cs ns2 (rename_vars_CAction1 lst a1) (rename_vars_CAction1 lst a2))
-rename_vars_CAction1 lst (CSPParal cs a1 a2)
- = (CSPParal cs (rename_vars_CAction1 lst a1) (rename_vars_CAction1 lst a2))
-rename_vars_CAction1 lst (CSPNSInter ns1 ns2 a1 a2)
- = (CSPNSInter ns1 ns2 (rename_vars_CAction1 lst a1) (rename_vars_CAction1 lst a2))
-rename_vars_CAction1 lst (CSPInterleave a1 a2)
- = (CSPInterleave (rename_vars_CAction1 lst a1) (rename_vars_CAction1 lst a2))
-rename_vars_CAction1 lst (CSPHide a cs)
- = (CSPHide (rename_vars_CAction1 lst a) cs)
-rename_vars_CAction1 lst (CSPParAction zn zexprls)
- = (CSPParAction zn (map (rename_vars_ZExpr1 lst) zexprls))
-rename_vars_CAction1 lst (CSPRenAction zn crpl)
- = (CSPRenAction zn (rename_vars_CReplace1 lst crpl))
-rename_vars_CAction1 lst (CSPRecursion zn a)
- = (CSPRecursion zn (rename_vars_CAction1 lst a))
-rename_vars_CAction1 lst (CSPUnParAction zgf a zn)
- = (CSPUnParAction zgf (rename_vars_CAction1 lst a) zn)
-rename_vars_CAction1 lst (CSPRepSeq zgf a)
- = (CSPRepSeq zgf (rename_vars_CAction1 lst a))
-rename_vars_CAction1 lst (CSPRepExtChoice zgf a)
- = (CSPRepExtChoice zgf (rename_vars_CAction1 lst a))
-rename_vars_CAction1 lst (CSPRepIntChoice zgf a)
- = (CSPRepIntChoice zgf (rename_vars_CAction1 lst a))
-rename_vars_CAction1 lst (CSPRepParalNS cs zgf ns a)
- = (CSPRepParalNS cs zgf ns (rename_vars_CAction1 lst a))
-rename_vars_CAction1 lst (CSPRepParal cs zgf a)
- = (CSPRepParal cs zgf (rename_vars_CAction1 lst a))
-rename_vars_CAction1 lst (CSPRepInterlNS zgf ns a)
- = (CSPRepInterlNS zgf ns (rename_vars_CAction1 lst a))
-rename_vars_CAction1 lst (CSPRepInterl zgf a)
- = (CSPRepInterl zgf (rename_vars_CAction1 lst a))
-
-
-
-rename_vars_Comm1 :: [(ZName, ZVar, ZExpr)] -> Comm -> Comm
-rename_vars_Comm1 lst (ChanComm zn cpls)
- = (ChanComm zn (map (rename_vars_CParameter1 lst) cpls))
-rename_vars_Comm1 lst (ChanGenComm zn zexprls cpls)
- = (ChanGenComm zn (map (rename_vars_ZExpr1 lst) zexprls) (map (rename_vars_CParameter1 lst) cpls))
-
-
-
-rename_vars_CParameter1 :: [(ZName, ZVar, ZExpr)] -> CParameter -> CParameter
-rename_vars_CParameter1 lst (ChanInp zn)
- = case (inListVar1 zn lst) of
-  True -> (ChanInp (join_name (get_proc_name zn lst) zn))
-  _ -> (ChanInp zn)
-rename_vars_CParameter1 lst (ChanInpPred zn zp)
- = case (inListVar1 zn lst) of
-  True -> (ChanInpPred (join_name (get_proc_name zn lst) zn) (rename_vars_ZPred1 lst zp))
-  _ -> (ChanInpPred zn zp)
-rename_vars_CParameter1 lst (ChanOutExp ze)
- = (ChanOutExp (rename_vars_ZExpr1 lst ze))
-rename_vars_CParameter1 lst (ChanDotExp ze)
- = (ChanDotExp (rename_vars_ZExpr1 lst ze))
-
-
-
-rename_vars_CCommand1 :: [(ZName, ZVar, ZExpr)] -> CCommand -> CCommand
-rename_vars_CCommand1 lst (CAssign zvarls1 zexprls)
- = (CAssign zvarls1 (map (rename_vars_ZExpr1 lst) zexprls))
-rename_vars_CCommand1 lst (CIf ga)
- = (CIf (rename_vars_CGActions1 lst ga))
-rename_vars_CCommand1 lst (CVarDecl zgf a)
- = (CVarDecl zgf (rename_vars_CAction1 lst a))
-rename_vars_CCommand1 lst (CAssumpt znls zp1 zp2)
- = (CAssumpt znls (rename_vars_ZPred1 lst zp1) zp2)
-rename_vars_CCommand1 lst (CAssumpt1 znls zp)
- = (CAssumpt1 znls zp)
-rename_vars_CCommand1 lst (CPrefix zp1 zp2)
- = (CPrefix (rename_vars_ZPred1 lst zp1) zp2)
-rename_vars_CCommand1 lst (CPrefix1 zp)
- = (CPrefix1 zp)
-rename_vars_CCommand1 lst (CommandBrace zp)
- = (CommandBrace zp)
-rename_vars_CCommand1 lst (CommandBracket zp)
- = (CommandBracket zp)
-rename_vars_CCommand1 lst (CValDecl zgf a)
- = (CValDecl zgf (rename_vars_CAction1 lst a))
-rename_vars_CCommand1 lst (CResDecl zgf a)
- = (CResDecl zgf (rename_vars_CAction1 lst a))
-rename_vars_CCommand1 lst (CVResDecl zgf a)
- = (CVResDecl zgf (rename_vars_CAction1 lst a))
-
-
-
-rename_vars_CGActions1 :: [(ZName, ZVar, ZExpr)] -> CGActions -> CGActions
-rename_vars_CGActions1 lst (CircGAction zp a)
- = (CircGAction (rename_vars_ZPred1 lst zp) (rename_vars_CAction1 lst a))
-rename_vars_CGActions1 lst (CircThenElse cga1 cga2)
- = (CircThenElse (rename_vars_CGActions1 lst cga1) (rename_vars_CGActions1 lst cga2))
-rename_vars_CGActions1 lst (CircElse pa)
- = (CircElse pa)
-
-
-
-rename_vars_CReplace1 :: [(ZName, ZVar, ZExpr)] -> CReplace -> CReplace
-rename_vars_CReplace1 lst (CRename zvarls1 zvarls)
- = (CRename zvarls1 zvarls)
-rename_vars_CReplace1 lst (CRenameAssign zvarls1 zvarls)
- = (CRenameAssign zvarls1 zvarls)
-
-
-
-bindingsVar1 lst []
- = []
-bindingsVar1 lst [((va,x),b)]
- = [(((join_name (get_proc_name va lst) va),x),(rename_vars_ZExpr1 lst b))]
-bindingsVar1 lst (((va,x),b):xs) 
- = [(((join_name (get_proc_name va lst) va),x),(rename_vars_ZExpr1 lst b))]++(bindingsVar1 lst xs)
-
-
-
-inListVar1 :: ZName -> [(ZName, ZVar, ZExpr)] -> Bool
-inListVar1 x []
- = False
-inListVar1 x [(a,(va,x1),b)]
- = case x == va of
-  True -> True
-  _ -> False
-inListVar1 x ((a,(va,x1),b):vst)
- = case x == va of
-  True -> True
-  _ -> inListVar1 x vst
-
-
-
-get_proc_name :: ZName -> [(ZName, ZVar, ZExpr)] -> ZName
-get_proc_name x [(a,(va,x1),b)]
- = case x == va of
-  True -> a
-  _ -> ""
-get_proc_name x ((a,(va,x1),b):vst)
- = case x == va of
-  True -> a
-  _ -> get_proc_name x vst
-
-
-
-rename_vars_ZExpr1 :: [(ZName, ZVar, ZExpr)] -> ZExpr -> ZExpr
-rename_vars_ZExpr1 lst (ZVar (va,x))
- = case (inListVar1 va lst) of
-  True -> (ZVar ((join_name (get_proc_name va lst) va),x))
-  _ -> (ZVar (va,x))
-rename_vars_ZExpr1 lst (ZInt zi)
- = (ZInt zi)
-rename_vars_ZExpr1 lst (ZGiven gv)
- = (ZGiven gv)
-rename_vars_ZExpr1 lst (ZFree0 va)
- = (ZFree0 va)
-rename_vars_ZExpr1 lst (ZFree1 va xpr)
- = (ZFree1 va (rename_vars_ZExpr1 lst xpr))
-rename_vars_ZExpr1 lst (ZTuple xpr)
- = (ZTuple (map (rename_vars_ZExpr1 lst) xpr))
-rename_vars_ZExpr1 lst (ZBinding xs)
- = (ZBinding (bindingsVar1 lst xs))
-rename_vars_ZExpr1 lst (ZSetDisplay xpr)
- = (ZSetDisplay (map (rename_vars_ZExpr1 lst) xpr))
-rename_vars_ZExpr1 lst (ZSeqDisplay xpr)
- = (ZSeqDisplay (map (rename_vars_ZExpr1 lst) xpr))
-rename_vars_ZExpr1 lst (ZFSet zf)
- = (ZFSet zf)
-rename_vars_ZExpr1 lst (ZIntSet i1 i2)
- = (ZIntSet i1 i2)
-rename_vars_ZExpr1 lst (ZGenerator zrl xpr)
- = (ZGenerator zrl (rename_vars_ZExpr1 lst xpr))
-rename_vars_ZExpr1 lst (ZCross xpr)
- = (ZCross (map (rename_vars_ZExpr1 lst) xpr))
-rename_vars_ZExpr1 lst (ZFreeType va pname1)
- = (ZFreeType va pname1)
-rename_vars_ZExpr1 lst (ZPowerSet{baseset=xpr, is_non_empty=b1, is_finite=b2})
- = (ZPowerSet{baseset=(rename_vars_ZExpr1 lst xpr), is_non_empty=b1, is_finite=b2})
-rename_vars_ZExpr1 lst (ZFuncSet{ domset=expr1, ranset=expr2, is_function=b1, is_total=b2, is_onto=b3, is_one2one=b4, is_sequence=b5, is_non_empty=b6, is_finite=b7})
- = (ZFuncSet{ domset=(rename_vars_ZExpr1 lst expr1), ranset=(rename_vars_ZExpr1 lst expr2), is_function=b1, is_total=b2, is_onto=b3, is_one2one=b4, is_sequence=b5, is_non_empty=b6, is_finite=b7})
-rename_vars_ZExpr1 lst (ZSetComp pname1 (Just xpr)) 
- = (ZSetComp pname1 (Just (rename_vars_ZExpr1 lst xpr)))
-rename_vars_ZExpr1 lst (ZSetComp pname1 Nothing) 
- = (ZSetComp pname1 Nothing)
-rename_vars_ZExpr1 lst (ZLambda pname1 xpr)
- = (ZLambda pname1 (rename_vars_ZExpr1 lst xpr))
-rename_vars_ZExpr1 lst (ZESchema zxp)
- = (ZESchema zxp)
-rename_vars_ZExpr1 lst (ZGivenSet gs)
- = (ZGivenSet gs)
-rename_vars_ZExpr1 lst (ZUniverse)
- = (ZUniverse)
-rename_vars_ZExpr1 lst (ZCall xpr1 xpr2)
- = (ZCall (rename_vars_ZExpr1 lst xpr1) (rename_vars_ZExpr1 lst xpr2))
-rename_vars_ZExpr1 lst (ZReln rl)
- = (ZReln rl)
-rename_vars_ZExpr1 lst (ZFunc1 f1)
- = (ZFunc1 f1)
-rename_vars_ZExpr1 lst (ZFunc2 f2)
- = (ZFunc2 f2)
-rename_vars_ZExpr1 lst (ZStrange st)
- = (ZStrange st)
-rename_vars_ZExpr1 lst (ZMu pname1 (Just xpr))
- = (ZMu pname1 (Just (rename_vars_ZExpr1 lst xpr)))
-rename_vars_ZExpr1 lst (ZELet pname1 xpr1)
- = (ZELet (bindingsVar1 lst pname1) (rename_vars_ZExpr1 lst xpr1))
-rename_vars_ZExpr1 lst (ZIf_Then_Else zp xpr1 xpr2)
- = (ZIf_Then_Else zp (rename_vars_ZExpr1 lst xpr1) (rename_vars_ZExpr1 lst xpr2))
-rename_vars_ZExpr1 lst (ZSelect xpr va)
- = (ZSelect xpr va)
-rename_vars_ZExpr1 lst (ZTheta zs)
- = (ZTheta zs)
-
-
-
-rename_vars_ZPred1 :: [(ZName, ZVar, ZExpr)] -> ZPred -> ZPred
-rename_vars_ZPred1 lst (ZFalse{reason=a})
- = (ZFalse{reason=a})
-rename_vars_ZPred1 lst (ZTrue{reason=a})
- = (ZTrue{reason=a})
-rename_vars_ZPred1 lst (ZAnd p1 p2)
- = (ZAnd (rename_vars_ZPred1 lst p1) (rename_vars_ZPred1 lst p2))
-rename_vars_ZPred1 lst (ZOr p1 p2)
- = (ZOr (rename_vars_ZPred1 lst p1) (rename_vars_ZPred1 lst p2))
-rename_vars_ZPred1 lst (ZImplies p1 p2)
- = (ZImplies (rename_vars_ZPred1 lst p1) (rename_vars_ZPred1 lst p2))
-rename_vars_ZPred1 lst (ZIff p1 p2)
- = (ZIff (rename_vars_ZPred1 lst p1) (rename_vars_ZPred1 lst p2))
-rename_vars_ZPred1 lst (ZNot p)
- = (ZNot (rename_vars_ZPred1 lst p))
-rename_vars_ZPred1 lst (ZExists pname1 p)
- = (ZExists pname1 (rename_vars_ZPred1 lst p))
-rename_vars_ZPred1 lst (ZExists_1 lst1 p)
- = (ZExists_1 lst1 (rename_vars_ZPred1 lst p))
-rename_vars_ZPred1 lst (ZForall pname1 p)
- = (ZForall pname1 (rename_vars_ZPred1 lst p))
-rename_vars_ZPred1 lst (ZPLet varxp p)
- = (ZPLet varxp (rename_vars_ZPred1 lst p))
-rename_vars_ZPred1 lst (ZEqual xpr1 xpr2)
- = (ZEqual (rename_vars_ZExpr1 lst xpr1) (rename_vars_ZExpr1 lst xpr2))
-rename_vars_ZPred1 lst (ZMember xpr1 xpr2)
- = (ZMember (rename_vars_ZExpr1 lst xpr1) (rename_vars_ZExpr1 lst xpr2))
-rename_vars_ZPred1 lst (ZPre sp)
- = (ZPre sp)
-rename_vars_ZPred1 lst (ZPSchema sp)
- = (ZPSchema sp)
-
-
-
--- extract the delta variables in here'
-get_delta_names [(ZFreeTypeDef ("NAME",[]) xs)]
-  = get_delta_names_aux xs
-get_delta_names ((ZFreeTypeDef ("NAME",[]) xs):xss) 
-  = (get_delta_names_aux xs)++(get_delta_names xss)
-get_delta_names (_:xs) 
-  = (get_delta_names xs)
-get_delta_names [] 
-  = []
-
-
-
-get_delta_names_aux [(ZBranch0 (a,[]))]
-  = [a]
-get_delta_names_aux ((ZBranch0 (a,[])):xs)
-  = [a]++(get_delta_names_aux xs)
-
-
-
-def_U_NAME x = ("U_"++(map toUpper (take 3 x)))
-def_U_prefix x = (map toTitle (take 3 x))
-
-mk_universe [] 
-  = ""
-mk_universe [(a,b,c,d)] 
-  = c++"."++d
-mk_universe ((a,b,c,d):xs)
-  = c++"."++d++" | "++(mk_universe xs)
-
-mk_subtype [] 
-  = ""
-mk_subtype [(a,b,c,d)] 
-  = "subtype "++b++" = "++c++"."++d++"\n"
-mk_subtype ((a,b,c,d):xs)
-  = "subtype "++b++" = "++c++"."++d++"\n"++(mk_subtype xs)
-
-mk_value [] 
-  = ""
-mk_value [(a,b,c,d)] 
-  = "value("++c++".v) = v\n"
-mk_value ((a,b,c,d):xs)
-  = "value("++c++".v) = v\n"++(mk_value xs)
-
-mk_type [] 
-  = ""
-mk_type [(a,b,c,d)] 
-  = a++" then "++b
-mk_type ((a,b,c,d):xs)
-  = a++" then "++b++"\n\t else if x == "++(mk_type xs)
-
-mk_tag [] 
-  = ""
-mk_tag [(a,b,c,d)] 
-  = a++" then "++c
-mk_tag ((a,b,c,d):xs)
-  = a++" then "++c++"\n\t else if x == "++(mk_tag xs)
-
-
-
--- extract the delta variables and types in here'
-def_universe [(ZAbbreviation ("\\delta",[]) (ZSetDisplay xs))]
-  = def_universe_aux xs
-def_universe ((ZAbbreviation ("\\delta",[]) (ZSetDisplay xs)):xss) 
-  = (def_universe_aux xs)++(def_universe xss)
-def_universe (_:xs) 
-  = (def_universe xs)
-def_universe [] 
-  = []
-
-
-
-def_universe_aux []
-  = [] 
-def_universe_aux [ZCall (ZVar ("\\mapsto",[])) (ZTuple [ZVar (b,[]),ZVar ("\\nat",[])])] = [(b,"U_NAT", "Nat", "NatValue")]
-def_universe_aux [ZCall (ZVar ("\\mapsto",[])) (ZTuple [ZVar (b,[]),ZVar (c,[])])] = [(b,(def_U_NAME c), (def_U_prefix c), c)]
-def_universe_aux ((ZCall (ZVar ("\\mapsto",[])) (ZTuple [ZVar (b,[]),ZVar ("\\nat",[])])):xs) = ((b,"U_NAT", "Nat", "NatValue"):(def_universe_aux xs))
-def_universe_aux ((ZCall (ZVar ("\\mapsto",[])) (ZTuple [ZVar (b,[]),ZVar (c,[])])):xs) = ((b,(def_U_NAME c), (def_U_prefix c), c):(def_universe_aux xs))
-
-
-
-filter_types_universe [(a,b,c,d)] = [(b,b,c,d)]
-filter_types_universe ((a,b,c,d):xs) = ((b,b,c,d):(filter_types_universe xs))
--- \end{code}
-
-
--- From Data.list
 
 -- | The 'union' function returns the list union of the two lists.
 -- For example,
@@ -1121,7 +359,6 @@ intersect               =  intersectBy (==)
 intersectBy             :: (a -> a -> Bool) -> [a] -> [a] -> [a]
 intersectBy eq xs ys    =  [x | x <- xs, any (eq x) ys]
 
-
 -- | /O(n^2)/. The 'nub' function removes duplicate elements from a list.
 -- In particular, it keeps only the first occurrence of each element.
 -- (The name 'nub' means \`essence\'.)
@@ -1137,15 +374,27 @@ nub l                   = nub' l []             -- '
         | otherwise     = x : nub' xs (x:ls)    -- '
 
 
--- | The 'genericTake' function is an overloaded version of 'take', which
--- accepts any 'Integral' value as the number of elements to take.
-take             :: (Integral i) => i -> [a] -> [a]
-take n _ | n <= 0 = []
-take _ []        =  []
-take n (x:xs)    =  x : take (n-1) xs
+-- | The 'nubBy' function behaves just like 'nub', except it uses a
+-- user-supplied equality predicate instead of the overloaded '=='
+-- function.
+nubBy                   :: (a -> a -> Bool) -> [a] -> [a]
+#ifdef USE_REPORT_PRELUDE
+nubBy eq []             =  []
+nubBy eq (x:xs)         =  x : nubBy eq (filter (\ y -> not (eq x y)) xs)
+#else
+nubBy eq l              = nubBy' l []
+  where
+    nubBy' [] _         = []
+    nubBy' (y:ys) xs
+       | elem_by eq y xs = nubBy' ys xs
+       | otherwise       = y : nubBy' ys (y:xs)
 
-
-
-toLower c = chr (fromIntegral (towlower (fromIntegral (ord c))))
-toUpper c = chr (fromIntegral (towupper (fromIntegral (ord c))))
-toTitle c = chr (fromIntegral (towtitle (fromIntegral (ord c))))
+-- Not exported:
+-- Note that we keep the call to `eq` with arguments in the
+-- same order as in the reference implementation
+-- 'xs' is the list of things we've seen so far, 
+-- 'y' is the potential new element
+elem_by :: (a -> a -> Bool) -> a -> [a] -> Bool
+elem_by _  _ []         =  False
+elem_by eq y (x:xs)     =  y `eq` x || elem_by eq y xs
+#endif
