test_haskabelle/MappingFunStatelessCircus.hs
@@ -19,114 +19,226 @@ omega_CAction :: [(ZName, ZVar, ZExpr)] -> CAction -> CAction
 omega_CAction lst CSPSkip = CSPSkip
 omega_CAction lst CSPStop = CSPStop
 omega_CAction lst CSPChaos = CSPChaos
-omega_CAction lst (CSPCommAction (ChanComm c []) a)
-  = (CSPCommAction (ChanComm c []) (omega_CAction lst a))
-omega_CAction lst (CSPCommAction (ChanComm c ((ChanOutExp e):xs)) a)
-  = omega_CAction lst (CSPCommAction (ChanComm c ((ChanDotExp e):xs)) a)
-omega_CAction lst (CSPSeq ca cb)
-  = (CSPSeq (omega_CAction lst ca) (omega_CAction lst cb))
-omega_CAction lst (CSPIntChoice ca cb)
-  = (CSPIntChoice (omega_CAction lst ca) (omega_CAction lst cb))
-
-
-
-
-omega_CAction lst (CSPCommAction (ChanComm c []) a)
-  = (CSPCommAction (ChanComm c []) (omega_CAction lst a))
-
-
+omega_CAction lst (CSPCommAction (ChanComm c []) a) = (CSPCommAction (ChanComm c []) (omega_CAction lst a))
+omega_CAction lst (CSPCommAction (ChanComm c ((ChanOutExp e):xs)) a) = omega_CAction lst (CSPCommAction (ChanComm c ((ChanDotExp e):xs)) a)
+omega_CAction lst (CSPSeq ca cb) = (CSPSeq (omega_CAction lst ca) (omega_CAction lst cb))
+omega_CAction lst (CSPIntChoice ca cb) = (CSPIntChoice (omega_CAction lst ca) (omega_CAction lst cb))
+omega_CAction lst (CSPCommAction (ChanComm c []) a) = (CSPCommAction (ChanComm c []) (omega_CAction lst a))
 omega_CAction lst (CSPHide a cs) = (CSPHide (omega_CAction lst a) cs)
-
-
-
 omega_CAction lst (CSPRecursion x c) = (CSPRecursion x (omega_CAction lst c))
+omega_CAction lst (CActionCommand (CommandBrace g)) = omega_CAction lst (CActionCommand (CPrefix g (ZTrue {reason = []})))
+omega_CAction lst (CActionCommand (CommandBracket g)) = omega_CAction lst (CActionCommand (CPrefix1 g))
+omega_CAction lst (CSPRenAction a (CRenameAssign left right)) = (CSPRenAction a (CRename right left))
+omega_CAction lst (CSPRepSeq [Choose (x,[]) (ZSeqDisplay xs)] (CSPParAction act [ZVar (x1,[])]))
+  = case x == x1 of
+    True -> omega_CAction lst (rep_CSPRepSeq lst act xs)
+    _  -> (CSPRepSeq [Choose (x,[]) (ZSeqDisplay xs)]
+          (omega_CAction lst (CSPParAction act [ZVar (x1,[])])))
+omega_CAction lst (CSPRepSeq [Choose (x,[]) v] act)
+  = (CSPRepSeq [Choose (x,[]) v] (omega_CAction lst act))
+
+omega_CAction lst (CSPRepExtChoice [Choose (x,[]) (ZSeqDisplay xs)] (CSPParAction act [ZVar (x1,[])]))
+  = case x == x1 of
+    True -> rep_CSPRepExtChoice lst act xs
+    _  -> (CSPRepExtChoice [Choose (x,[]) (ZSeqDisplay xs)]
+          (CSPParAction act [ZVar (x1,[])]))
+omega_CAction lst (CSPRepExtChoice [Choose (x,[]) v]
+          act)
+  = (CSPRepExtChoice [Choose (x,[]) v] (omega_CAction lst act))
+
+omega_CAction lst (CSPRepIntChoice [Choose (x,[]) (ZSeqDisplay xs)]
+          (CSPParAction act [ZVar (x1,[])]))
+  = case x == x1 of
+    True -> rep_CSPRepIntChoice lst act xs
+    _  -> (CSPRepIntChoice [Choose (x,[]) (ZSeqDisplay xs)]
+          (CSPParAction act [ZVar (x1,[])]))
+omega_CAction lst (CSPRepIntChoice [Choose (x,[]) v] act)
+  = (CSPRepIntChoice [Choose (x,[]) v] (omega_CAction lst act))
+
+omega_CAction lst (CSPRepParalNS (CSExpr cs) [Choose (x,[]) (ZSetDisplay lsx)]
+          (NSExprParam ns [ZVar (x1,[])])
+          (CSPParAction a [ZVar (x2,[])]))
+  = case (x == x1) && (x == x2) of
+    True -> rep_CSPRepParalNS lst a cs ns x lsx
+    _  -> (CSPRepParalNS (CSExpr cs) [Choose (x,[]) (ZSetDisplay lsx)]
+          (NSExprParam ns [ZVar (x1,[])])
+          (omega_CAction lst (CSPParAction a [ZVar (x2,[])])))
+omega_CAction lst (CSPRepParalNS (CSExpr cs) [Choose (x,[]) (ZSetDisplay lsx)]
+          (NSExprParam ns [ZVar (x1,[])]) act)
+  = (CSPRepParalNS (CSExpr cs) [Choose (x,[]) (ZSetDisplay lsx)]
+          (NSExprParam ns [ZVar (x1,[])])
+          (omega_CAction lst act))
+omega_CAction lst (CSPRepInterlNS [Choose (x,[]) (ZSetDisplay lsx)]
+          (NSExprParam ns [ZVar (x1,[])])
+          (CSPParAction a [ZVar (x2,[])]))
+  = case (x == x1) && (x == x2) of
+    True -> rep_CSPRepInterlNS lst a ns x lsx
+    _  ->  (CSPRepInterlNS [Choose (x,[]) (ZSetDisplay lsx)]
+          (NSExprParam ns [ZVar (x1,[])])
+          (omega_CAction lst (CSPParAction a [ZVar (x2,[])])))
+omega_CAction lst (CSPRepInterlNS [Choose (x,[]) (ZSetDisplay lsx)]
+          (NSExprParam ns [ZVar (x1,[])])
+          act)
+  = (CSPRepInterlNS [Choose (x,[]) (ZSetDisplay lsx)]
+          (NSExprParam ns [ZVar (x1,[])])
+          (omega_CAction lst act))
+
+omega_CAction lst (CActionCommand (CIf (CircGAction g a)))
+  = make_get_com lst lsx (rename_vars_CAction (map fst lsx) (CActionCommand
+             (CIf (CircGAction g (omega_prime_CAction lst a)))))
+  where
+   lsx = free_var_ZPred g
+
+omega_CAction lst (CSPCommAction (ChanComm c ((ChanDotExp e):xs)) a)
+  = make_get_com lst lxs (rename_vars_CAction (map fst lxs) (CSPCommAction (ChanComm c ((ChanDotExp e):xs)) (omega_prime_CAction lst a)))
+  where lxs = (get_chan_param ((ChanDotExp e):xs)) `intersect` (filter_state_comp lst)
+
+omega_CAction lst (CActionCommand (CAssign varls valls)) 
+  = make_get_com lst varls (rename_vars_CAction (map fst (filter_state_comp lst)) (make_set_com lst varls valls CSPSkip))
 
 
+omega_CAction lst (CActionCommand (CIf (CircThenElse gl glx)))
+  = make_get_com lst lsx (rename_vars_CAction (map fst lsx) (CActionCommand (CIf (mk_guard_pair lst guard_pair))))
+  where
+   guard_pair = get_guard_pair (CircThenElse gl glx)
+   lsx = nub $ concat $ map free_var_ZPred (map fst guard_pair)
 
 
-omega_CAction lst (CActionCommand (CommandBrace g))
-  = omega_CAction lst (CActionCommand (CPrefix g (ZTrue {reason = []})))
-
-
-
-omega_CAction lst (CActionCommand (CommandBracket g))
-  = omega_CAction lst (CActionCommand (CPrefix1 g))
-
-
-
-omega_CAction lst (CSPRenAction a (CRenameAssign left right))
-  = (CSPRenAction a (CRename right left))
-omega_CAction lst x = x
 -- Omega Prime
 
 omega_prime_CAction :: [(ZName, ZVar, ZExpr)] -> CAction -> CAction
 omega_prime_CAction lst CSPSkip = CSPSkip
-omega_prime_CAction lst CSPStop = CSPStop
 omega_prime_CAction lst CSPChaos = CSPChaos
-
-
-omega_prime_CAction lst (CSPCommAction (ChanComm c []) a)
-  = (CSPCommAction (ChanComm c []) (omega_prime_CAction lst a))
-
-
-
-omega_prime_CAction lst (CSPCommAction (ChanComm c x) a)
-  = (CSPCommAction (ChanComm c x) (omega_prime_CAction lst a))
-
-
-
-omega_prime_CAction lst (CSPGuard g a)
-  = (CSPGuard g (omega_prime_CAction lst a))
-
-
-
-omega_prime_CAction lst (CSPSeq ca cb)
-  = (CSPSeq (omega_prime_CAction lst ca) (omega_prime_CAction lst cb))
-
-
-
-omega_prime_CAction lst (CSPIntChoice ca cb)
-  = (CSPIntChoice (omega_prime_CAction lst ca) (omega_prime_CAction lst cb))
-
-
-omega_prime_CAction lst (CActionCommand (CIf (CircGAction g a)))
-  = (CActionCommand (CIf (CircGAction g (omega_prime_CAction lst a))))
-
-
+omega_prime_CAction lst CSPStop = CSPStop
+omega_prime_CAction lst (CActionCommand (CAssign varls valls)) = (make_set_com lst varls valls CSPSkip)
+omega_prime_CAction lst (CActionCommand (CIf (CircGAction g a))) = (CActionCommand (CIf (CircGAction g (omega_prime_CAction lst a))))
+omega_prime_CAction lst (CActionCommand (CommandBrace g)) = omega_prime_CAction lst (CActionCommand (CPrefix g (ZTrue {reason = []})))
+omega_prime_CAction lst (CActionCommand (CommandBracket g)) = omega_prime_CAction lst (CActionCommand (CPrefix1 g))
+omega_prime_CAction lst (CActionName n) = (CActionName n)
+omega_prime_CAction lst (CSPCommAction (ChanComm c []) a) = (CSPCommAction (ChanComm c []) (omega_prime_CAction lst a))
+omega_prime_CAction lst (CSPCommAction (ChanComm c x) a) = (CSPCommAction (ChanComm c x) (omega_prime_CAction lst a))
+omega_prime_CAction lst (CSPGuard g a) = (CSPGuard g (omega_prime_CAction lst a))
 omega_prime_CAction lst (CSPHide a cs) = (CSPHide (omega_prime_CAction lst a) cs)
-
-
-
+omega_prime_CAction lst (CSPIntChoice ca cb) = (CSPIntChoice (omega_prime_CAction lst ca) (omega_prime_CAction lst cb))
 omega_prime_CAction lst (CSPRecursion x c) = (CSPRecursion x (omega_prime_CAction lst c))
+omega_prime_CAction lst (CSPRenAction a (CRenameAssign left right)) = (CSPRenAction a (CRename right left))
+omega_prime_CAction lst (CSPRepIntChoice [Choose (x,[]) v] act) = (CSPRepIntChoice [Choose (x,[]) v] (omega_prime_CAction lst act))
+omega_prime_CAction lst (CSPRepSeq [Choose (x,[]) v] act) = (CSPRepSeq [Choose (x,[]) v] (omega_prime_CAction lst act))
+omega_prime_CAction lst (CSPSeq ca cb) = (CSPSeq (omega_prime_CAction lst ca) (omega_prime_CAction lst cb))
 
+omega_prime_CAction lst (CActionCommand (CIf (CircThenElse gl glx)))
+  = (CActionCommand (CIf (mk_guard_pair lst guard_pair)))
+  where
+   guard_pair = get_guard_pair (CircThenElse gl glx)
 
+omega_prime_CAction lst (CSPRepInterlNS [Choose (x,[]) (ZSetDisplay lsx)]
+          (NSExprParam ns [ZVar (x1,[])])
+          (CSPParAction a [ZVar (x2,[])]))
+  = case (x == x1) && (x == x2) of
+    True -> rep_CSPRepInterlNS lst a ns x lsx
+    _  ->  (CSPRepInterlNS [Choose (x,[]) (ZSetDisplay lsx)]
+          (NSExprParam ns [ZVar (x1,[])])
+          (omega_prime_CAction lst (CSPParAction a [ZVar (x2,[])])))
+omega_prime_CAction lst (CSPRepInterlNS [Choose (x,[]) (ZSetDisplay lsx)]
+          (NSExprParam ns [ZVar (x1,[])])
+          act)
+  = (CSPRepInterlNS [Choose (x,[]) (ZSetDisplay lsx)]
+          (NSExprParam ns [ZVar (x1,[])])
+          (omega_prime_CAction lst act))
 
-omega_prime_CAction lst (CActionCommand (CommandBrace g))
-  = omega_prime_CAction lst (CActionCommand (CPrefix g (ZTrue {reason = []})))
+omega_prime_CAction lst (CSPRepParalNS (CSExpr cs) [Choose (x,[]) (ZSetDisplay lsx)]
+          (NSExprParam ns [ZVar (x1,[])])
+          (CSPParAction a [ZVar (x2,[])]))
+  = case (x == x1) && (x == x2) of
+    True -> rep_CSPRepParalNS lst a cs ns x lsx
+    _  -> (CSPRepParalNS (CSExpr cs) [Choose (x,[]) (ZSetDisplay lsx)]
+          (NSExprParam ns [ZVar (x1,[])])
+          (omega_prime_CAction lst (CSPParAction a [ZVar (x2,[])])))
+omega_prime_CAction lst (CSPRepParalNS (CSExpr cs) [Choose (x,[]) (ZSetDisplay lsx)]
+          (NSExprParam ns [ZVar (x1,[])]) act)
+  = (CSPRepParalNS (CSExpr cs) [Choose (x,[]) (ZSetDisplay lsx)]
+          (NSExprParam ns [ZVar (x1,[])])
+          (omega_prime_CAction lst act))
 
+omega_prime_CAction lst (CSPRepSeq [Choose (x,[]) (ZSeqDisplay xs)] (CSPParAction act [ZVar (x1,[])]))
+  = case x == x1 of
+    True -> omega_prime_CAction lst (rep_CSPRepSeq lst act xs)
+    _  -> (CSPRepSeq [Choose (x,[]) (ZSeqDisplay xs)]
+          (omega_prime_CAction lst (CSPParAction act [ZVar (x1,[])])))
+omega_prime_CAction lst (CSPRepExtChoice [Choose (x,[]) (ZSeqDisplay xs)] (CSPParAction act [ZVar (x1,[])]))
+  = case x == x1 of
+    True -> rep_CSPRepExtChoice lst act xs
+    _  -> (CSPRepExtChoice [Choose (x,[]) (ZSeqDisplay xs)]
+          (CSPParAction act [ZVar (x1,[])]))
 
-
-omega_prime_CAction lst (CActionCommand (CommandBracket g))
-  = omega_prime_CAction lst (CActionCommand (CPrefix1 g))
-
-
-
-omega_prime_CAction lst (CSPRenAction a (CRenameAssign left right))
-  = (CSPRenAction a (CRename right left))
-
-
-
-omega_prime_CAction lst (CActionName n)
-  = (CActionName n)
-
-
-
-omega_prime_CAction lst x 
-  = error ("Not defined for Omega'"++ show x)
-
-
+omega_prime_CAction lst (CSPRepIntChoice [Choose (x,[]) (ZSeqDisplay xs)]
+          (CSPParAction act [ZVar (x1,[])]))
+  = case x == x1 of
+    True -> rep_CSPRepIntChoice lst act xs
+    _  -> (CSPRepIntChoice [Choose (x,[]) (ZSeqDisplay xs)]
+          (CSPParAction act [ZVar (x1,[])]))
 
 -- Extra from MappingFunStatelesssCircus.lhs
+rep_CSPRepSeq :: [(ZName, ZVar, ZExpr)] -> ZName -> [ZExpr] -> CAction
+rep_CSPRepSeq lst a [x]
+  = omega_CAction lst (CSPParAction a [x])
+rep_CSPRepSeq lst a (x:xs)
+  = CSPSeq (omega_CAction lst (CSPParAction a [x])) (rep_CSPRepSeq lst a xs)
+
+rep_CSPRepIntChoice :: [(ZName, ZVar, ZExpr)] -> ZName -> [ZExpr] -> CAction
+rep_CSPRepIntChoice lst a [x]
+  = omega_CAction lst (CSPParAction a [x])
+rep_CSPRepIntChoice lst a (x:xs)
+  = CSPIntChoice (omega_CAction lst (CSPParAction a [x])) (rep_CSPRepIntChoice lst a xs)
+
+rep_CSPRepExtChoice :: [(ZName, ZVar, ZExpr)] -> ZName -> [ZExpr] -> CAction
+rep_CSPRepExtChoice lst a [x]
+  =  omega_CAction lst (CSPParAction a [x])
+rep_CSPRepExtChoice lst a (x:xs)
+  = CSPExtChoice ( omega_CAction lst (CSPParAction a [x])) (rep_CSPRepExtChoice lst a xs)
+
+rep_CSPRepParalNS :: [(ZName, ZVar, ZExpr)] -> ZName -> ZName -> ZName -> String -> [ZExpr] -> CAction
+rep_CSPRepParalNS lst a _ _ _ [x]
+  =  omega_CAction lst (CSPParAction a [x])
+rep_CSPRepParalNS lst a cs ns y (x:xs)
+  = (CSPNSParal (NSExprParam ns [x]) (CSExpr cs)
+    (NSBigUnion (ZSetComp
+           [Choose (y,[]) (ZSetDisplay xs)]
+           (Just (ZCall (ZVar (ns,[])) (ZVar (y,[])))) ) )
+     ( omega_CAction lst (CSPParAction a [x])) (rep_CSPRepParalNS lst a cs ns y xs) )
+
+rep_CSPRepInterlNS :: [(ZName, ZVar, ZExpr)] -> ZName -> ZName -> String -> [ZExpr] -> CAction
+rep_CSPRepInterlNS lst a _ _ [x]
+  =  omega_CAction lst (CSPParAction a [x])
+rep_CSPRepInterlNS lst a ns y (x:xs)
+  = (CSPNSInter (NSExprParam ns [x])
+    (NSBigUnion (ZSetComp
+           [Choose (y,[]) (ZSetDisplay xs)]
+           (Just (ZCall (ZVar (ns,[])) (ZVar (y,[])))) ) )
+     ( omega_CAction lst (CSPParAction a [x])) (rep_CSPRepInterlNS lst a ns y xs) )
+
+-- 
+
+filter_state_comp :: [(ZName, ZVar, ZExpr)] -> [ZVar]
+filter_state_comp [] = []
+filter_state_comp [(_, v, _)] = [v]
+filter_state_comp ((_, v, _):xs) = [v]++(filter_state_comp xs)
+
+get_guard_pair :: CGActions -> [(ZPred, CAction)]
+get_guard_pair (CircThenElse (CircGAction g2 a2) (CircGAction g3 a3)) = [(g2,a2),(g3,a3)]
+get_guard_pair (CircThenElse (CircGAction g1 a1) glx) = [(g1,a1)]++(get_guard_pair glx)
+
+
+mk_guard_pair :: [(ZName, ZVar, ZExpr)] -> [(ZPred, CAction)] -> CGActions
+mk_guard_pair lst [(g,a)] = (CircGAction g (omega_prime_CAction lst a))
+mk_guard_pair lst ((g,a):ls) = (CircThenElse (CircGAction g (omega_prime_CAction lst a)) (mk_guard_pair lst ls))
+
+
+make_get_com :: [(ZName, ZVar, ZExpr)] -> [ZVar] -> CAction -> CAction
+make_get_com lst [(x,[])] c = (CSPCommAction (ChanComm "mget"[ChanDotExp (ZVar ((get_proc_name x lst)++"_"++x,[])),ChanInp ("v"++(get_proc_name x lst)++"_"++x)]) c)
+make_get_com lst ((x,[]):xs) c = (CSPCommAction (ChanComm "mget"[ChanDotExp (ZVar ((get_proc_name x lst)++"_"++x,[])),ChanInp ("v"++(get_proc_name x lst)++"_"++x)]) (make_get_com lst xs c))
+make_get_com lst x c = c   
+
 get_proc_name :: ZName -> [(ZName, ZVar, ZExpr)] -> ZName
 get_proc_name x [(a,(va,x1),b)]
  = case x == va of
@@ -137,258 +249,227 @@ get_proc_name x ((a,(va,x1),b):vst)
   True -> a
   _ -> get_proc_name x vst
 
-make_get_com :: [(ZName, ZVar, ZExpr)] -> [ZVar] -> CAction -> CAction
-make_get_com lst [(x,[])] c
-  = (CSPCommAction (ChanComm "mget"
-    [ChanDotExp (ZVar ((get_proc_name x lst)++"_"++x,[])),ChanInp ("v"++(get_proc_name x lst)++"_"++x)]) c)
-make_get_com lst ((x,[]):xs) c
-  = (CSPCommAction (ChanComm "mget"
-    [ChanDotExp (ZVar ((get_proc_name x lst)++"_"++x,[])),ChanInp ("v"++(get_proc_name x lst)++"_"++x)]) (make_get_com lst xs c))
-make_get_com lst x c = c   
 
--- Extra from DefSets.hs
-
-filter_state_comp :: [(ZName, ZVar, ZExpr)] -> [ZVar]
-filter_state_comp [] = []
-filter_state_comp [(_, v, _)] = [v]
-filter_state_comp ((_, v, _):xs) = [v]++(filter_state_comp xs)
-
-get_chan_param :: [CParameter] -> [ZVar]
-get_chan_param [] = [] 
-get_chan_param [ChanDotExp (ZVar (x,_))] 
- = [(x,[])]
-get_chan_param [ChanOutExp (ZVar (x,_))] 
- = [(x,[])]
-get_chan_param [_] 
- = []
-get_chan_param ((ChanDotExp (ZVar (x,_))):xs) 
- = [(x,[])]++(get_chan_param xs)
-get_chan_param ((ChanOutExp (ZVar (x,_))):xs) 
- = [(x,[])]++(get_chan_param xs)
-get_chan_param (_:xs) = (get_chan_param xs)
+make_set_com :: [(ZName, ZVar, ZExpr)] -> [ZVar] -> [ZExpr] -> CAction -> CAction
+make_set_com lst [(x,[])] [y] c = (CSPCommAction (ChanComm "mset"[ChanDotExp (ZVar ((get_proc_name x lst)++"_"++x,[])),ChanOutExp y]) (omega_CAction lst c))
+make_set_com lst (((x,[])):xs) (y:ys) c = (CSPCommAction (ChanComm "mset"[ChanDotExp (ZVar ((get_proc_name x lst)++"_"++x,[])),ChanOutExp y]) (make_set_com lst xs ys c))
 
 
-rename_vars_CAction lst (CActionSchemaExpr zsexp)
- = (CActionSchemaExpr zsexp)
-rename_vars_CAction lst (CActionCommand cmd)
- = (CActionCommand (rename_vars_CCommand lst cmd))
-rename_vars_CAction lst (CActionName zn)
- = (CActionName zn)
-rename_vars_CAction lst (CSPSkip )
- = (CSPSkip )
-rename_vars_CAction lst (CSPStop )
- = (CSPStop )
-rename_vars_CAction lst (CSPChaos)
- = (CSPChaos)
-rename_vars_CAction lst (CSPCommAction c a)
- = (CSPCommAction (rename_vars_Comm lst c) (rename_vars_CAction lst a))
-rename_vars_CAction lst (CSPGuard zp a)
- = (CSPGuard (rename_ZPred lst zp) (rename_vars_CAction lst a))
-rename_vars_CAction lst (CSPSeq a1 a2)
- = (CSPSeq (rename_vars_CAction lst a1) (rename_vars_CAction lst a2))
-rename_vars_CAction lst (CSPExtChoice a1 a2)
- = (CSPExtChoice (rename_vars_CAction lst a1) (rename_vars_CAction lst a2))
-rename_vars_CAction lst (CSPIntChoice a1 a2)
- = (CSPIntChoice (rename_vars_CAction lst a1) (rename_vars_CAction lst a2))
-rename_vars_CAction lst (CSPNSParal ns1 cs ns2 a1 a2)
- = (CSPNSParal ns1 cs ns2 (rename_vars_CAction lst a1) (rename_vars_CAction lst a2))
-rename_vars_CAction lst (CSPParal cs a1 a2)
- = (CSPParal cs (rename_vars_CAction lst a1) (rename_vars_CAction lst a2))
-rename_vars_CAction lst (CSPNSInter ns1 ns2 a1 a2)
- = (CSPNSInter ns1 ns2 (rename_vars_CAction lst a1) (rename_vars_CAction lst a2))
-rename_vars_CAction lst (CSPInterleave a1 a2)
- = (CSPInterleave (rename_vars_CAction lst a1) (rename_vars_CAction lst a2))
-rename_vars_CAction lst (CSPHide a cs)
- = (CSPHide (rename_vars_CAction lst a) cs)
-rename_vars_CAction lst (CSPParAction zn zexprls)
- = (CSPParAction zn (map (rename_ZExpr lst) zexprls))
-rename_vars_CAction lst (CSPRenAction zn crpl)
- = (CSPRenAction zn (rename_vars_CReplace lst crpl))
-rename_vars_CAction lst (CSPRecursion zn a)
- = (CSPRecursion zn (rename_vars_CAction lst a))
-rename_vars_CAction lst (CSPUnParAction zgf a zn)
- = (CSPUnParAction zgf (rename_vars_CAction lst a) zn)
-rename_vars_CAction lst (CSPRepSeq zgf a)
- = (CSPRepSeq zgf (rename_vars_CAction lst a))
-rename_vars_CAction lst (CSPRepExtChoice zgf a)
- = (CSPRepExtChoice zgf (rename_vars_CAction lst a))
-rename_vars_CAction lst (CSPRepIntChoice zgf a)
- = (CSPRepIntChoice zgf (rename_vars_CAction lst a))
-rename_vars_CAction lst (CSPRepParalNS cs zgf ns a)
- = (CSPRepParalNS cs zgf ns (rename_vars_CAction lst a))
-rename_vars_CAction lst (CSPRepParal cs zgf a)
- = (CSPRepParal cs zgf (rename_vars_CAction lst a))
-rename_vars_CAction lst (CSPRepInterlNS zgf ns a)
- = (CSPRepInterlNS zgf ns (rename_vars_CAction lst a))
-rename_vars_CAction lst (CSPRepInterl zgf a)
- = (CSPRepInterl zgf (rename_vars_CAction lst a))
+-- All that should be found in the Defsets.hs file
+
+getWrtV xs = []
+
+free_var_CAction :: CAction -> [ZVar]
+free_var_CAction (CActionCommand c) = (free_var_comnd c)
+free_var_CAction (CSPCommAction (ChanComm com xs) c) = (get_chan_param xs)++(free_var_CAction c)
+free_var_CAction (CSPGuard p c) = (free_var_ZPred p)++(free_var_CAction c)
+free_var_CAction (CSPSeq ca cb) = (free_var_CAction ca)++(free_var_CAction cb)
+free_var_CAction (CSPExtChoice ca cb) = (free_var_CAction ca)++(free_var_CAction cb)
+free_var_CAction (CSPIntChoice ca cb) = (free_var_CAction ca)++(free_var_CAction cb)
+free_var_CAction (CSPNSParal ns1 cs ns2 ca cb) = (free_var_CAction ca)++(free_var_CAction cb)
+free_var_CAction (CSPParal cs ca cb) = (free_var_CAction ca)++(free_var_CAction cb)
+free_var_CAction (CSPNSInter ns1 ns2 ca cb) = (free_var_CAction ca)++(free_var_CAction cb)
+free_var_CAction (CSPInterleave ca cb) = (free_var_CAction ca)++(free_var_CAction cb)
+free_var_CAction (CSPHide c cs) = (free_var_CAction c)
+free_var_CAction (CSPRecursion nm c) = (free_var_CAction c)
+free_var_CAction (CSPUnParAction lst c nm) = (free_var_CAction c) \\ (fvs free_var_ZGenFilt lst)
+free_var_CAction (CSPRepSeq lst c) = (free_var_CAction c) \\ (fvs free_var_ZGenFilt lst)
+free_var_CAction (CSPRepExtChoice lst c) = (free_var_CAction c) \\ (fvs free_var_ZGenFilt lst)
+free_var_CAction (CSPRepIntChoice lst c) = (free_var_CAction c) \\ (fvs free_var_ZGenFilt lst)
+free_var_CAction (CSPRepParalNS cs lst ns c) = (free_var_CAction c) \\ (fvs free_var_ZGenFilt lst)
+free_var_CAction (CSPRepParal cs lst c) = (free_var_CAction c) \\ (fvs free_var_ZGenFilt lst)
+free_var_CAction (CSPRepInterlNS lst ns c) = (free_var_CAction c) \\ (fvs free_var_ZGenFilt lst)
+free_var_CAction (CSPRepInterl lst c) = (free_var_CAction c) \\ (fvs free_var_ZGenFilt lst)
+free_var_CAction _ = []
+
+free_var_ZGenFilt (Choose v e) = [v]
+free_var_ZGenFilt _ = []
+
+free_var_comnd (CAssign v e) = v
+free_var_comnd (CIf ga) = free_var_if ga
+free_var_comnd (CVarDecl z c) = (free_var_CAction c) \\ (fvs free_var_ZGenFilt z)
+free_var_comnd (CommandBrace z) = (free_var_ZPred z)
+free_var_comnd (CommandBracket z) = (free_var_ZPred z)
+free_var_comnd (CValDecl z c) = (free_var_CAction c) \\ (fvs free_var_ZGenFilt z)
+free_var_comnd (CResDecl z c) = (free_var_CAction c) \\ (fvs free_var_ZGenFilt z)
+free_var_comnd (CVResDecl z c) = (free_var_CAction c) \\ (fvs free_var_ZGenFilt z)
+free_var_comnd _ = []
+ 
+free_var_if (CircGAction p a) = (free_var_ZPred p)++(free_var_CAction a)
+free_var_if (CircThenElse ga gb) = (free_var_if ga)++(free_var_if gb)
+free_var_if (CircElse (CircusAction a)) = (free_var_CAction a)
+free_var_if (CircElse (ParamActionDecl x (CircusAction a))) = (free_var_CAction a) \\ (fvs free_var_ZGenFilt x)
 
 
+free_var_ZPred :: ZPred -> [ZVar]
+free_var_ZPred (ZFalse{reason=p})
+  = error "Don't know what free vars of ZFalse are right now. Check back later"
+free_var_ZPred (ZTrue{reason=p})
+  = error "Don't know what free vars of ZTrue are right now. Check back later"
+free_var_ZPred (ZAnd a b)
+ = free_var_ZPred a ++ free_var_ZPred b
+free_var_ZPred (ZOr a b)
+ = free_var_ZPred a ++ free_var_ZPred b
+free_var_ZPred (ZImplies a b)
+ = free_var_ZPred a ++ free_var_ZPred b
+free_var_ZPred (ZIff a b)
+ = free_var_ZPred a ++ free_var_ZPred b
+free_var_ZPred (ZNot a)
+ = free_var_ZPred a
+free_var_ZPred (ZExists [Choose v e] a)
+ = (free_var_ZPred a) \\ [v]
+free_var_ZPred (ZExists ls a)
+  = error "Don't know what free vars of ZExists are right now. Check back later"
+free_var_ZPred (ZExists_1 [Choose v e] a)
+ = (free_var_ZPred a) \\ [v]
+free_var_ZPred (ZExists_1 ls a)
+  = error "Don't know what free vars of ZExists_1 are right now. Check back later"
+free_var_ZPred (ZForall [Choose v e] a)
+ = (free_var_ZPred a) \\ [v]
+free_var_ZPred (ZForall ls a)
+  = error "Don't know what free vars of ZForall are right now. Check back later"
+free_var_ZPred (ZPLet ls a )
+   = error "Don't know what free vars of ZPLet are right now. Check back later"
+free_var_ZPred (ZEqual expa expb)
+ = free_var_ZExpr expa ++ free_var_ZExpr expb
+free_var_ZPred (ZMember expa expb)
+  = free_var_ZExpr expa
+free_var_ZPred (ZPre zsexpr)
+  = error "Don't know what free vars of ZPre are right now. Check back later"
+free_var_ZPred (ZPSchema zsexpr)
+  = error "Don't know what free vars of ZPSchema are right now. Check back later"
 
-rename_vars_Comm lst (ChanComm zn cpls)
- = (ChanComm zn (map (rename_vars_CParameter lst) cpls))
-rename_vars_Comm lst (ChanGenComm zn zexprls cpls)
- = (ChanGenComm zn (map (rename_ZExpr lst) zexprls) (map (rename_vars_CParameter lst) cpls))
+fvs f [] = []
+fvs f (e:es)
+ = f(e) ++ (fvs f (es))
 
-
-
-rename_vars_CParameter lst (ChanInp zn)
- = (ChanInp zn)
-rename_vars_CParameter lst (ChanInpPred zn zp)
- = (ChanInpPred zn (rename_ZPred lst zp))
-rename_vars_CParameter lst (ChanOutExp ze)
- = (ChanOutExp (rename_ZExpr lst ze))
-rename_vars_CParameter lst (ChanDotExp ze)
- = (ChanDotExp (rename_ZExpr lst ze))
-
-
-
-rename_vars_CCommand lst (CAssign zvarls1 zexprls)
- = (CAssign zvarls1 (map (rename_ZExpr lst) zexprls))
-rename_vars_CCommand lst (CIf ga)
- = (CIf (rename_vars_CGActions lst ga))
-rename_vars_CCommand lst (CVarDecl zgf a)
- = (CVarDecl zgf (rename_vars_CAction lst a))
-rename_vars_CCommand lst (CAssumpt znls zp1 zp2)
- = (CAssumpt znls (rename_ZPred lst zp1) zp2)
-rename_vars_CCommand lst (CAssumpt1 znls zp)
- = (CAssumpt1 znls zp)
-rename_vars_CCommand lst (CPrefix zp1 zp2)
- = (CPrefix (rename_ZPred lst zp1) zp2)
-rename_vars_CCommand lst (CPrefix1 zp)
- = (CPrefix1 zp)
-rename_vars_CCommand lst (CommandBrace zp)
- = (CommandBrace zp)
-rename_vars_CCommand lst (CommandBracket zp)
- = (CommandBracket zp)
-rename_vars_CCommand lst (CValDecl zgf a)
- = (CValDecl zgf (rename_vars_CAction lst a))
-rename_vars_CCommand lst (CResDecl zgf a)
- = (CResDecl zgf (rename_vars_CAction lst a))
-rename_vars_CCommand lst (CVResDecl zgf a)
- = (CVResDecl zgf (rename_vars_CAction lst a))
+free_var_ZExpr :: ZExpr -> [ZVar]
+free_var_ZExpr(ZVar v) = [v]
+free_var_ZExpr(ZInt c ) = []
+free_var_ZExpr(ZTuple exls ) = fvs free_var_ZExpr exls
+free_var_ZExpr(ZSetDisplay exls ) = fvs free_var_ZExpr exls
+free_var_ZExpr(ZSeqDisplay exls ) = fvs free_var_ZExpr exls
+free_var_ZExpr(ZCross exls ) = fvs free_var_ZExpr exls
+free_var_ZExpr(ZPowerSet{baseset=b, is_non_empty=e, is_finite=fs}) = error "Don't know what free vars of ZPowerSet are right now. Check back later"
+free_var_ZExpr(ZFuncSet{domset=d, ranset=r, is_function=f, is_total=t, is_onto=o, is_one2one=oo, is_sequence=s, is_non_empty=ne, is_finite=ff}) = error "Don't know what free vars of ZFree0 are right now. Check back later"
+free_var_ZExpr(ZLambda [Choose v e] a) = (free_var_ZExpr a) \\ [v]
+free_var_ZExpr(ZLambda _ a) = []
+free_var_ZExpr(ZCall ex ex2) = free_var_ZExpr ex2 -- is this right??
+free_var_ZExpr(ZELet ves pr) = ((free_var_ZExpr(pr)) \\ (map fst ves)) ++ fvs free_var_ZExpr (map snd ves)
+-- free_var_ZExpr(ZIf_Then_Else zp ex ex1) -- = free_var_ZPred zp ++ free_var_ZExpr ex ++ free_var_ZExpr ex1
+free_var_ZExpr(ZSelect ex zv) = free_var_ZExpr ex ++ [zv]
+free_var_ZExpr _ = []
 
 
 
-rename_vars_CGActions lst (CircGAction zp a)
- = (CircGAction (rename_ZPred lst zp) (rename_vars_CAction lst a))
-rename_vars_CGActions lst (CircThenElse cga1 cga2)
- = (CircThenElse (rename_vars_CGActions lst cga1) (rename_vars_CGActions lst cga2))
-rename_vars_CGActions lst (CircElse pa)
- = (CircElse pa)
+rename_vars_CAction lst (CActionSchemaExpr zsexp) = (CActionSchemaExpr zsexp)
+rename_vars_CAction lst (CActionCommand cmd) = (CActionCommand (rename_vars_CCommand lst cmd))
+rename_vars_CAction lst (CActionName zn) = (CActionName zn)
+rename_vars_CAction lst (CSPSkip ) = (CSPSkip )
+rename_vars_CAction lst (CSPStop ) = (CSPStop )
+rename_vars_CAction lst (CSPChaos) = (CSPChaos)
+rename_vars_CAction lst (CSPCommAction c a) = (CSPCommAction (rename_vars_Comm lst c) (rename_vars_CAction lst a))
+rename_vars_CAction lst (CSPGuard zp a) = (CSPGuard (rename_ZPred lst zp) (rename_vars_CAction lst a))
+rename_vars_CAction lst (CSPSeq a1 a2) = (CSPSeq (rename_vars_CAction lst a1) (rename_vars_CAction lst a2))
+rename_vars_CAction lst (CSPExtChoice a1 a2) = (CSPExtChoice (rename_vars_CAction lst a1) (rename_vars_CAction lst a2))
+rename_vars_CAction lst (CSPIntChoice a1 a2) = (CSPIntChoice (rename_vars_CAction lst a1) (rename_vars_CAction lst a2))
+rename_vars_CAction lst (CSPNSParal ns1 cs ns2 a1 a2) = (CSPNSParal ns1 cs ns2 (rename_vars_CAction lst a1) (rename_vars_CAction lst a2))
+rename_vars_CAction lst (CSPParal cs a1 a2) = (CSPParal cs (rename_vars_CAction lst a1) (rename_vars_CAction lst a2))
+rename_vars_CAction lst (CSPNSInter ns1 ns2 a1 a2) = (CSPNSInter ns1 ns2 (rename_vars_CAction lst a1) (rename_vars_CAction lst a2))
+rename_vars_CAction lst (CSPInterleave a1 a2) = (CSPInterleave (rename_vars_CAction lst a1) (rename_vars_CAction lst a2))
+rename_vars_CAction lst (CSPHide a cs) = (CSPHide (rename_vars_CAction lst a) cs)
+rename_vars_CAction lst (CSPParAction zn zexprls) = (CSPParAction zn (map (rename_ZExpr lst) zexprls))
+rename_vars_CAction lst (CSPRenAction zn crpl) = (CSPRenAction zn (rename_vars_CReplace lst crpl))
+rename_vars_CAction lst (CSPRecursion zn a) = (CSPRecursion zn (rename_vars_CAction lst a))
+rename_vars_CAction lst (CSPUnParAction zgf a zn) = (CSPUnParAction zgf (rename_vars_CAction lst a) zn)
+rename_vars_CAction lst (CSPRepSeq zgf a) = (CSPRepSeq zgf (rename_vars_CAction lst a))
+rename_vars_CAction lst (CSPRepExtChoice zgf a) = (CSPRepExtChoice zgf (rename_vars_CAction lst a))
+rename_vars_CAction lst (CSPRepIntChoice zgf a) = (CSPRepIntChoice zgf (rename_vars_CAction lst a))
+rename_vars_CAction lst (CSPRepParalNS cs zgf ns a) = (CSPRepParalNS cs zgf ns (rename_vars_CAction lst a))
+rename_vars_CAction lst (CSPRepParal cs zgf a) = (CSPRepParal cs zgf (rename_vars_CAction lst a))
+rename_vars_CAction lst (CSPRepInterlNS zgf ns a) = (CSPRepInterlNS zgf ns (rename_vars_CAction lst a))
+rename_vars_CAction lst (CSPRepInterl zgf a) = (CSPRepInterl zgf (rename_vars_CAction lst a))
+rename_vars_CAction lst x = x
 
+rename_vars_CCommand lst (CAssign zvarls1 zexprls) = (CAssign zvarls1 (map (rename_ZExpr lst) zexprls))
+rename_vars_CCommand lst (CIf ga) = (CIf (rename_vars_CGActions lst ga))
+rename_vars_CCommand lst (CVarDecl zgf a) = (CVarDecl zgf (rename_vars_CAction lst a))
+rename_vars_CCommand lst (CAssumpt znls zp1 zp2) = (CAssumpt znls (rename_ZPred lst zp1) zp2)
+rename_vars_CCommand lst (CAssumpt1 znls zp) = (CAssumpt1 znls zp)
+rename_vars_CCommand lst (CPrefix zp1 zp2) = (CPrefix (rename_ZPred lst zp1) zp2)
+rename_vars_CCommand lst (CPrefix1 zp) = (CPrefix1 zp)
+rename_vars_CCommand lst (CommandBrace zp) = (CommandBrace zp)
+rename_vars_CCommand lst (CommandBracket zp) = (CommandBracket zp)
+rename_vars_CCommand lst (CValDecl zgf a) = (CValDecl zgf (rename_vars_CAction lst a))
+rename_vars_CCommand lst (CResDecl zgf a) = (CResDecl zgf (rename_vars_CAction lst a))
+rename_vars_CCommand lst (CVResDecl zgf a) = (CVResDecl zgf (rename_vars_CAction lst a))
 
+rename_vars_CReplace lst (CRename zvarls1 zvarls) = (CRename zvarls1 zvarls)
+rename_vars_CReplace lst (CRenameAssign zvarls1 zvarls) = (CRenameAssign zvarls1 zvarls)
 
-rename_vars_CReplace lst (CRename zvarls1 zvarls)
- = (CRename zvarls1 zvarls)
-rename_vars_CReplace lst (CRenameAssign zvarls1 zvarls)
- = (CRenameAssign zvarls1 zvarls)
+rename_vars_Comm lst (ChanComm zn cpls) = (ChanComm zn (map (rename_vars_CParameter lst) cpls))
+rename_vars_Comm lst (ChanGenComm zn zexprls cpls) = (ChanGenComm zn (map (rename_ZExpr lst) zexprls) (map (rename_vars_CParameter lst) cpls))
 
+rename_vars_CParameter lst (ChanInp zn) = (ChanInp zn)
+rename_vars_CParameter lst (ChanInpPred zn zp) = (ChanInpPred zn (rename_ZPred lst zp))
+rename_vars_CParameter lst (ChanOutExp ze) = (ChanOutExp (rename_ZExpr lst ze))
+rename_vars_CParameter lst (ChanDotExp ze) = (ChanDotExp (rename_ZExpr lst ze))
 
-rename_ZVar lst (va,x)
-  = case (inListVar va lst) of
-     True -> ("v_"++va,x)
-     False -> (va,x)
+rename_vars_CGActions lst (CircGAction zp a) = (CircGAction (rename_ZPred lst zp) (rename_vars_CAction lst a))
+rename_vars_CGActions lst (CircThenElse cga1 cga2) = (CircThenElse (rename_vars_CGActions lst cga1) (rename_vars_CGActions lst cga2))
+rename_vars_CGActions lst (CircElse pa) = (CircElse pa)
+
 rename_ZExpr lst (ZVar (va,x))
  = case (inListVar va lst) of
    True -> (ZVar ("v_"++va,x))
    False -> (ZVar (va,x))
-rename_ZExpr lst (ZInt zi)
- = (ZInt zi)
-rename_ZExpr lst (ZGiven gv)
- = (ZGiven gv)
-rename_ZExpr lst (ZFree0 va)
- = (ZFree0 va)
-rename_ZExpr lst (ZFree1 va xpr)
- = (ZFree1 va (rename_ZExpr lst xpr))
-rename_ZExpr lst (ZTuple xprlst)
- = (ZTuple (map (rename_ZExpr lst) xprlst))
-rename_ZExpr lst (ZBinding xs)
- = (ZBinding (bindingsVar lst xs))
-rename_ZExpr lst (ZSetDisplay xprlst)
- = (ZSetDisplay (map (rename_ZExpr lst) xprlst))
-rename_ZExpr lst (ZSeqDisplay xprlst)
- = (ZSeqDisplay (map (rename_ZExpr lst) xprlst))
-rename_ZExpr lst (ZFSet zf)
- = (ZFSet zf)
-rename_ZExpr lst (ZIntSet i1 i2)
- = (ZIntSet i1 i2)
-rename_ZExpr lst (ZGenerator zrl xpr)
- = (ZGenerator zrl (rename_ZExpr lst xpr))
-rename_ZExpr lst (ZCross xprlst)
- = (ZCross (map (rename_ZExpr lst) xprlst))
-rename_ZExpr lst (ZFreeType va lst1)
- = (ZFreeType va lst1)
-rename_ZExpr lst (ZPowerSet{baseset=xpr, is_non_empty=b1, is_finite=b2})
- = (ZPowerSet{baseset=(rename_ZExpr lst xpr), is_non_empty=b1, is_finite=b2})
-rename_ZExpr lst (ZFuncSet{ domset=expr1, ranset=expr2, is_function=b1, is_total=b2, is_onto=b3, is_one2one=b4, is_sequence=b5, is_non_empty=b6, is_finite=b7})
- = (ZFuncSet{ domset=(rename_ZExpr lst expr1), ranset=(rename_ZExpr lst expr2), is_function=b1, is_total=b2, is_onto=b3, is_one2one=b4, is_sequence=b5, is_non_empty=b6, is_finite=b7})
-rename_ZExpr lst (ZSetComp lst1 (Just xpr)) 
- = (ZSetComp lst1 (Just (rename_ZExpr lst xpr)))
-rename_ZExpr lst (ZSetComp lst1 Nothing) 
- = (ZSetComp lst1 Nothing)
-rename_ZExpr lst (ZLambda lst1 xpr)
- = (ZLambda lst1 (rename_ZExpr lst xpr))
-rename_ZExpr lst (ZESchema zxp)
- = (ZESchema zxp)
-rename_ZExpr lst (ZGivenSet gs)
- = (ZGivenSet gs)
-rename_ZExpr lst (ZUniverse)
- = (ZUniverse)
-rename_ZExpr lst (ZCall xpr1 xpr2)
- = (ZCall (rename_ZExpr lst xpr1) (rename_ZExpr lst xpr2))
-rename_ZExpr lst (ZReln rl)
- = (ZReln rl)
-rename_ZExpr lst (ZFunc1 f1)
- = (ZFunc1 f1)
-rename_ZExpr lst (ZFunc2 f2)
- = (ZFunc2 f2)
-rename_ZExpr lst (ZStrange st)
- = (ZStrange st)
-rename_ZExpr lst (ZMu lst1 (Just xpr))
- = (ZMu lst1 (Just (rename_ZExpr lst xpr)))
-rename_ZExpr lst (ZELet lst1 xpr1)
- = (ZELet (bindingsVar lst lst1) (rename_ZExpr lst xpr1))
-rename_ZExpr lst (ZIf_Then_Else zp xpr1 xpr2)
- = (ZIf_Then_Else zp (rename_ZExpr lst xpr1) (rename_ZExpr lst xpr2))
-rename_ZExpr lst (ZSelect xpr va)
- = (ZSelect xpr va)
-rename_ZExpr lst (ZTheta zs)
- = (ZTheta zs)
+rename_ZExpr lst (ZInt zi) = (ZInt zi)
+rename_ZExpr lst (ZGiven gv) = (ZGiven gv)
+rename_ZExpr lst (ZFree0 va) = (ZFree0 va)
+rename_ZExpr lst (ZFree1 va xpr) = (ZFree1 va (rename_ZExpr lst xpr))
+rename_ZExpr lst (ZTuple xprlst) = (ZTuple (map (rename_ZExpr lst) xprlst))
+rename_ZExpr lst (ZBinding xs) = (ZBinding (bindingsVar lst xs))
+rename_ZExpr lst (ZSetDisplay xprlst) = (ZSetDisplay (map (rename_ZExpr lst) xprlst))
+rename_ZExpr lst (ZSeqDisplay xprlst) = (ZSeqDisplay (map (rename_ZExpr lst) xprlst))
+rename_ZExpr lst (ZFSet zf) = (ZFSet zf)
+rename_ZExpr lst (ZIntSet i1 i2) = (ZIntSet i1 i2)
+rename_ZExpr lst (ZGenerator zrl xpr) = (ZGenerator zrl (rename_ZExpr lst xpr))
+rename_ZExpr lst (ZCross xprlst) = (ZCross (map (rename_ZExpr lst) xprlst))
+rename_ZExpr lst (ZFreeType va lst1) = (ZFreeType va lst1)
+rename_ZExpr lst (ZPowerSet{baseset=xpr, is_non_empty=b1, is_finite=b2}) = (ZPowerSet{baseset=(rename_ZExpr lst xpr), is_non_empty=b1, is_finite=b2})
+rename_ZExpr lst (ZFuncSet{ domset=expr1, ranset=expr2, is_function=b1, is_total=b2, is_onto=b3, is_one2one=b4, is_sequence=b5, is_non_empty=b6, is_finite=b7}) = (ZFuncSet{ domset=(rename_ZExpr lst expr1), ranset=(rename_ZExpr lst expr2), is_function=b1, is_total=b2, is_onto=b3, is_one2one=b4, is_sequence=b5, is_non_empty=b6, is_finite=b7})
+rename_ZExpr lst (ZSetComp lst1 (Just xpr)) = (ZSetComp lst1 (Just (rename_ZExpr lst xpr)))
+rename_ZExpr lst (ZSetComp lst1 Nothing) = (ZSetComp lst1 Nothing)
+rename_ZExpr lst (ZLambda lst1 xpr) = (ZLambda lst1 (rename_ZExpr lst xpr))
+rename_ZExpr lst (ZESchema zxp) = (ZESchema zxp)
+rename_ZExpr lst (ZGivenSet gs) = (ZGivenSet gs)
+rename_ZExpr lst (ZUniverse) = (ZUniverse)
+rename_ZExpr lst (ZCall xpr1 xpr2) = (ZCall (rename_ZExpr lst xpr1) (rename_ZExpr lst xpr2))
+rename_ZExpr lst (ZReln rl) = (ZReln rl)
+rename_ZExpr lst (ZFunc1 f1) = (ZFunc1 f1)
+rename_ZExpr lst (ZFunc2 f2) = (ZFunc2 f2)
+rename_ZExpr lst (ZStrange st) = (ZStrange st)
+rename_ZExpr lst (ZMu lst1 (Just xpr)) = (ZMu lst1 (Just (rename_ZExpr lst xpr)))
+rename_ZExpr lst (ZELet lst1 xpr1) = (ZELet (bindingsVar lst lst1) (rename_ZExpr lst xpr1))
+rename_ZExpr lst (ZIf_Then_Else zp xpr1 xpr2) = (ZIf_Then_Else zp (rename_ZExpr lst xpr1) (rename_ZExpr lst xpr2))
+rename_ZExpr lst (ZSelect xpr va) = (ZSelect xpr va)
+rename_ZExpr lst (ZTheta zs) = (ZTheta zs)
 
-
-
-rename_ZPred lst (ZFalse{reason=a})
- = (ZFalse{reason=a})
-rename_ZPred lst (ZTrue{reason=a})
- = (ZTrue{reason=a})
-rename_ZPred lst (ZAnd p1 p2)
- = (ZAnd (rename_ZPred lst p1) (rename_ZPred lst p2))
-rename_ZPred lst (ZOr p1 p2)
- = (ZOr (rename_ZPred lst p1) (rename_ZPred lst p2))
-rename_ZPred lst (ZImplies p1 p2)
- = (ZImplies (rename_ZPred lst p1) (rename_ZPred lst p2))
-rename_ZPred lst (ZIff p1 p2)
- = (ZIff (rename_ZPred lst p1) (rename_ZPred lst p2))
-rename_ZPred lst (ZNot p)
- = (ZNot (rename_ZPred lst p))
-rename_ZPred lst (ZExists lst1 p)
- = (ZExists lst1 (rename_ZPred lst p))
-rename_ZPred lst (ZExists_1 lst1 p)
- = (ZExists_1 lst1 (rename_ZPred lst p))
-rename_ZPred lst (ZForall lst1 p)
- = (ZForall lst1 (rename_ZPred lst p))
-rename_ZPred lst (ZPLet varxp p)
- = (ZPLet varxp (rename_ZPred lst p))
-rename_ZPred lst (ZEqual xpr1 xpr2)
- = (ZEqual (rename_ZExpr lst xpr1) (rename_ZExpr lst xpr2))
-rename_ZPred lst (ZMember xpr1 xpr2)
- = (ZMember (rename_ZExpr lst xpr1) (rename_ZExpr lst xpr2))
-rename_ZPred lst (ZPre sp)
- = (ZPre sp)
-rename_ZPred lst (ZPSchema sp)
- = (ZPSchema sp)
-
+rename_ZPred lst (ZFalse{reason=a}) = (ZFalse{reason=a})
+rename_ZPred lst (ZTrue{reason=a}) = (ZTrue{reason=a})
+rename_ZPred lst (ZAnd p1 p2) = (ZAnd (rename_ZPred lst p1) (rename_ZPred lst p2))
+rename_ZPred lst (ZOr p1 p2) = (ZOr (rename_ZPred lst p1) (rename_ZPred lst p2))
+rename_ZPred lst (ZImplies p1 p2) = (ZImplies (rename_ZPred lst p1) (rename_ZPred lst p2))
+rename_ZPred lst (ZIff p1 p2) = (ZIff (rename_ZPred lst p1) (rename_ZPred lst p2))
+rename_ZPred lst (ZNot p) = (ZNot (rename_ZPred lst p))
+rename_ZPred lst (ZExists lst1 p) = (ZExists lst1 (rename_ZPred lst p))
+rename_ZPred lst (ZExists_1 lst1 p) = (ZExists_1 lst1 (rename_ZPred lst p))
+rename_ZPred lst (ZForall lst1 p) = (ZForall lst1 (rename_ZPred lst p))
+rename_ZPred lst (ZPLet varxp p) = (ZPLet varxp (rename_ZPred lst p))
+rename_ZPred lst (ZEqual xpr1 xpr2) = (ZEqual (rename_ZExpr lst xpr1) (rename_ZExpr lst xpr2))
+rename_ZPred lst (ZMember xpr1 xpr2) = (ZMember (rename_ZExpr lst xpr1) (rename_ZExpr lst xpr2))
+rename_ZPred lst (ZPre sp) = (ZPre sp)
+rename_ZPred lst (ZPSchema sp) = (ZPSchema sp)
 
 inListVar x []
  = False
@@ -400,8 +481,6 @@ inListVar x (va:vst)
  = case x == va of
   True -> True
   _ -> inListVar x vst
-
-
 
 
 bindingsVar lst []
@@ -416,9 +495,74 @@ bindingsVar lst (((va,x),b):xs)
    False -> [((va,x),(rename_ZExpr lst b))]++(bindingsVar lst xs)
 
 
+get_chan_param :: [CParameter] -> [ZVar]
+get_chan_param [] = [] 
+get_chan_param [ChanDotExp (ZVar (x,_))] = [(x,[])]
+get_chan_param [ChanOutExp (ZVar (x,_))] = [(x,[])]
+get_chan_param [_] = []
+get_chan_param ((ChanDotExp (ZVar (x,_))):xs) = [(x,[])]++(get_chan_param xs)
+get_chan_param ((ChanOutExp (ZVar (x,_))):xs) = [(x,[])]++(get_chan_param xs)
+get_chan_param (_:xs) = (get_chan_param xs)
 
--- From Data.list
 
+-- Artur - 15/12/2016
+-- What we find below this line was taken from the Data.List module
+-- It is hard to import such package with Haskabelle, so I had
+-- to put it directly into my code.
+
+-- From Data.List
+-- | The '\\' function is list difference ((non-associative).
+-- In the result of @xs@ '\\' @ys@, the first occurrence of each element of
+-- @ys@ in turn (if any) has been removed from @xs@.  Thus
+--
+-- > (xs ++ ys) \\ xs == ys.
+--
+-- It is a special case of 'deleteFirstsBy', which allows the programmer
+-- to supply their own equality test.
+
+(\\)                    :: (Eq a) => [a] -> [a] -> [a]
+(\\)                    =  foldl (flip delete)
+
+
+-- | 'delete' @x@ removes the first occurrence of @x@ from its list argument.
+-- For example,
+--
+-- > delete 'a' "banana" == "bnana"
+--
+-- It is a special case of 'deleteBy', which allows the programmer to
+-- supply their own equality test.
+
+delete                  :: (Eq a) => a -> [a] -> [a]
+delete                  =  deleteBy (==)
+
+-- | The 'deleteBy' function behaves like 'delete', but takes a
+-- user-supplied equality predicate.
+deleteBy                :: (a -> a -> Bool) -> a -> [a] -> [a]
+deleteBy _  _ []        = []
+deleteBy eq x (y:ys)    = if x `eq` y then ys else y : deleteBy eq x ys
+
+
+flip         :: (a -> b -> c) -> b -> a -> c
+flip f x y   =  f y x
+
+
+-- | The 'union' function returns the list union of the two lists.
+-- For example,
+--
+-- > "dog" `union` "cow" == "dogcw"
+--
+-- Duplicates, and elements of the first list, are removed from the
+-- the second list, but if the first list contains duplicates, so will
+-- the result.
+-- It is a special case of 'unionBy', which allows the programmer to supply
+-- their own equality test.
+
+union                   :: (Eq a) => [a] -> [a] -> [a]
+union                   = unionBy (==)
+
+-- | The 'unionBy' function is the non-overloaded version of 'union'.
+unionBy                 :: (a -> a -> Bool) -> [a] -> [a] -> [a]
+unionBy eq xs ys        =  xs ++ foldl (flip (deleteBy eq)) (nubBy eq ys) xs
 
 -- | The 'intersect' function takes the list intersection of two lists.
 -- For example,
@@ -439,7 +583,6 @@ intersect               =  intersectBy (==)
 intersectBy             :: (a -> a -> Bool) -> [a] -> [a] -> [a]
 intersectBy eq xs ys    =  [x | x <- xs, any (eq x) ys]
 
-
 -- | /O(n^2)/. The 'nub' function removes duplicate elements from a list.
 -- In particular, it keeps only the first occurrence of each element.
 -- (The name 'nub' means \`essence\'.)
@@ -454,9 +597,28 @@ nub l                   = nub' l []             -- '
         | x `elem` ls   = nub' xs ls            -- '
         | otherwise     = x : nub' xs (x:ls)    -- '
 
--- | The 'genericTake' function is an overloaded version of 'take', which
--- accepts any 'Integral' value as the number of elements to take.
-take             :: (Integral i) => i -> [a] -> [a]
-take n _ | n <= 0 = []
-take _ []        =  []
-take n (x:xs)    =  x : take (n-1) xs
+
+-- | The 'nubBy' function behaves just like 'nub', except it uses a
+-- user-supplied equality predicate instead of the overloaded '=='
+-- function.
+nubBy                   :: (a -> a -> Bool) -> [a] -> [a]
+#ifdef USE_REPORT_PRELUDE
+nubBy eq []             =  []
+nubBy eq (x:xs)         =  x : nubBy eq (filter (\ y -> not (eq x y)) xs)
+#else
+nubBy eq l              = nubBy' l []
+  where
+    nubBy' [] _         = []
+    nubBy' (y:ys) xs
+       | elem_by eq y xs = nubBy' ys xs
+       | otherwise       = y : nubBy' ys (y:xs)
+
+-- Not exported:
+-- Note that we keep the call to `eq` with arguments in the
+-- same order as in the reference implementation
+-- 'xs' is the list of things we've seen so far, 
+-- 'y' is the potential new element
+elem_by :: (a -> a -> Bool) -> a -> [a] -> Bool
+elem_by _  _ []         =  False
+elem_by eq y (x:xs)     =  y `eq` x || elem_by eq y xs
+#endif
